wip: Main

src/Main.fst
@@ -29,6 +29,19 @@ open Config
 open Utils2
 open Mman
 
+module G = FStar.Ghost
+
+
+let metadata_max_ex = SlabsCommon2.metadata_max_ex
+
+let slab_size = SlabsCommon2.slab_size
+
+// Size of the slab region for one size class
+// metadata_max * page_size
+// ==
+// metadata_max_ex * slab_size
+let sc_slab_region_size = SlabsCommon2.slab_region_size
+
 #push-options  "--ide_id_info_off"
 (**  Handwritten mmap functions to allocate basic data structures *)
 
@@ -50,8 +63,6 @@ val intro_ind_varraylist_nil (#opened:_)
         Seq.index s 6 == 0sz
       )
       (ensures fun _ _ _ -> True)
-
-module G = FStar.Ghost
 
 let intro_ind_varraylist_nil r r_idxs =
   ALG.intro_arraylist_nil #AL.status
@@ -92,6 +103,66 @@ let intro_ind_varraylist_nil r r_idxs =
     (A.varray r_idxs)
     (SlabsCommon.ind_varraylist_aux r idxs)
     (SlabsCommon.ind_varraylist_aux r)
+
+val intro_ind_varraylist_nil2 (#opened:_)
+  (r: A.array AL.cell)
+  (r_idxs: A.array US.t{A.length r_idxs = 7})
+  : SteelGhost unit opened
+      (A.varray r `star` A.varray r_idxs)
+      (fun _ -> SlabsCommon2.ind_varraylist r r_idxs)
+      (requires fun h ->
+        let s : Seq.lseq US.t 7 = A.asel r_idxs h in
+        A.length r == 0 /\
+        Seq.index s 0 == AL.null_ptr /\
+        Seq.index s 1 == AL.null_ptr /\
+        Seq.index s 2 == AL.null_ptr /\
+        Seq.index s 3 == AL.null_ptr /\
+        Seq.index s 4 == AL.null_ptr /\
+        Seq.index s 5 == AL.null_ptr /\
+        Seq.index s 6 == 0sz
+      )
+      (ensures fun _ _ _ -> True)
+
+let intro_ind_varraylist_nil2 r r_idxs =
+  let open SlabsCommon2 in
+  ALG.intro_arraylist_nil
+    pred1 pred2 pred3 pred4 pred5
+    r
+    AL.null_ptr
+    AL.null_ptr
+    AL.null_ptr
+    AL.null_ptr
+    AL.null_ptr
+    AL.null_ptr
+    0sz;
+  let idxs
+    : G.erased (Seq.lseq US.t 7)
+    = gget (A.varray r_idxs) in
+  ind_varraylist_aux2_lemma r idxs
+      AL.null_ptr
+      AL.null_ptr
+      AL.null_ptr
+      AL.null_ptr
+      AL.null_ptr
+      AL.null_ptr
+      0sz;
+  change_equal_slprop
+    (AL.varraylist pred1 pred2 pred3 pred4 pred5 r
+      (US.v AL.null_ptr)
+      (US.v AL.null_ptr)
+      (US.v AL.null_ptr)
+      (US.v AL.null_ptr)
+      (US.v AL.null_ptr)
+      (US.v AL.null_ptr)
+      (US.v 0sz))
+    (ind_varraylist_aux2 r idxs);
+  intro_vrefine
+    (SlabsCommon2.ind_varraylist_aux2 r idxs)
+    (SlabsCommon2.ind_varraylist_aux_refinement r idxs);
+  intro_vdep
+    (A.varray r_idxs)
+    (SlabsCommon2.ind_varraylist_aux r idxs)
+    (SlabsCommon2.ind_varraylist_aux r)
 
 val intro_left_vprop_empty (#opened:_)
   (sc:sc)
@@ -158,6 +229,75 @@ let intro_left_vprop_empty sc slab_region md_bm_region md_region r_idxs
       r_idxs)
     (left_vprop2 sc slab_region md_bm_region md_region r_idxs 0sz s)
     (left_vprop2 sc slab_region md_bm_region md_region r_idxs 0sz)
+#pop-options
+
+val intro_left_vprop_empty2 (#opened:_)
+  (sc:sc_ex)
+  (slab_region: array U8.t{A.length slab_region = US.v metadata_max_ex * US.v slab_size})
+  (md_bm_region: array bool{A.length md_bm_region = US.v metadata_max_ex})
+  (md_region: array AL.cell{A.length md_region = US.v metadata_max_ex})
+  (r_idxs: A.array US.t{A.length r_idxs = 7})
+  : SteelGhost unit opened
+      (A.varray (split_l md_region 0sz) `star`
+      A.varray r_idxs)
+      (fun _ -> SlabsCommon2.left_vprop sc slab_region md_bm_region md_region r_idxs 0sz)
+      (requires fun h ->
+        let s : Seq.lseq US.t 7 = A.asel r_idxs h in
+        Seq.index s 0 == AL.null_ptr /\
+        Seq.index s 1 == AL.null_ptr /\
+        Seq.index s 2 == AL.null_ptr /\
+        Seq.index s 3 == AL.null_ptr /\
+        Seq.index s 4 == AL.null_ptr /\
+        Seq.index s 5 == AL.null_ptr /\
+        Seq.index s 6 == 0sz
+      )
+      (ensures fun _ _ _ -> True)
+
+#push-options "--z3rlimit 50"
+let intro_left_vprop_empty2 sc slab_region md_bm_region md_region r_idxs
+  =
+  let open SlabsCommon2 in
+  intro_ind_varraylist_nil2
+    (A.split_l md_region 0sz)
+    r_idxs;
+  let s = gget (ind_varraylist
+      (A.split_l md_region 0sz)
+      r_idxs) in
+
+  starseq_intro_empty #_
+      #(pos:US.t{US.v pos < US.v 0sz})
+      #(SlabsCommon2.t sc)
+      (SlabsCommon2.f sc slab_region md_bm_region 0sz (ALG.dataify (dsnd s)))
+      (SlabsCommon2.f_lemma sc slab_region md_bm_region 0sz (ALG.dataify (dsnd s)))
+      (SeqUtils.init_us_refined (US.v 0sz));
+
+  assert (SeqUtils.init_us_refined (US.v 0sz) `Seq.equal` Seq.empty);
+
+  let open FStar.Tactics in
+  assert ((starseq
+      #(pos:US.t{US.v pos < US.v 0sz})
+      #(t sc)
+      (f sc slab_region md_bm_region 0sz (ALG.dataify (dsnd s)))
+      (f_lemma sc slab_region md_bm_region 0sz (ALG.dataify (dsnd s)))
+      (SeqUtils.init_us_refined (US.v 0sz))) ==
+    (left_vprop2 sc slab_region md_bm_region md_region r_idxs 0sz s))
+  by (norm [delta_only [`%left_vprop2]]);
+
+  change_equal_slprop
+    (starseq
+      #(pos:US.t{US.v pos < US.v 0sz})
+      #(t sc)
+      (f sc slab_region md_bm_region 0sz (ALG.dataify (dsnd s)))
+      (f_lemma sc slab_region md_bm_region 0sz (ALG.dataify (dsnd s)))
+      (SeqUtils.init_us_refined (US.v 0sz)))
+    (left_vprop2 sc slab_region md_bm_region md_region r_idxs 0sz s);
+  intro_vdep
+    (ind_varraylist
+      (A.split_l md_region 0sz)
+      r_idxs)
+    (left_vprop2 sc slab_region md_bm_region md_region r_idxs 0sz s)
+    (left_vprop2 sc slab_region md_bm_region md_region r_idxs 0sz)
+#pop-options
 
 val intro_right_vprop_empty (#opened:_)
   (slab_region: array U8.t{A.length slab_region = US.v metadata_max * U32.v page_size})
@@ -199,6 +339,44 @@ let intro_right_vprop_empty slab_region md_bm_region md_region =
     A.varray (A.split_r md_region 0sz))
     (right_vprop slab_region md_bm_region md_region 0sz)
 
+val intro_right_vprop_empty2 (#opened:_)
+  (slab_region: array U8.t{A.length slab_region = US.v metadata_max_ex * US.v slab_size})
+  (md_bm_region: array bool{A.length md_bm_region = US.v metadata_max_ex})
+  (md_region: array AL.cell{A.length md_region = US.v metadata_max_ex})
+  : SteelGhost unit opened
+     (A.varray (split_r slab_region 0sz) `star`
+      A.varray (split_r md_bm_region 0sz) `star`
+      A.varray (split_r md_region 0sz))
+    (fun _ -> SlabsCommon2.right_vprop slab_region md_bm_region md_region 0sz)
+    (requires fun h ->
+      A.asel (split_r slab_region 0sz) h `Seq.equal` Seq.create (A.length slab_region) U8.zero /\
+      A.asel (split_r md_bm_region 0sz) h `Seq.equal` Seq.create (A.length md_bm_region) false)
+    (ensures fun _ _ _ -> True)
+
+let intro_right_vprop_empty2 slab_region md_bm_region md_region =
+  let open SlabsCommon2 in
+  change_equal_slprop
+    (A.varray (A.split_r slab_region 0sz))
+    (A.varray (A.split_r slab_region (US.mul 0sz slab_size)));
+  intro_vrefine
+    (A.varray (A.split_r slab_region (US.mul 0sz slab_size))) zf_u8;
+  intro_vrefine
+    (A.varray (A.split_r md_bm_region 0sz)) zf_b;
+  assert_norm (
+    (A.varray (A.split_r slab_region (US.mul 0sz slab_size))
+      `vrefine` zf_u8) `star`
+    (A.varray (A.split_r md_bm_region 0sz)
+      `vrefine` zf_b) `star`
+    A.varray (A.split_r md_region 0sz) ==
+    (right_vprop slab_region md_bm_region md_region 0sz));
+  change_equal_slprop
+    ((A.varray (A.split_r slab_region (US.mul 0sz slab_size))
+      `vrefine` zf_u8) `star`
+    (A.varray (A.split_r md_bm_region 0sz)
+      `vrefine` zf_b) `star`
+    A.varray (A.split_r md_region 0sz))
+    (right_vprop slab_region md_bm_region md_region 0sz)
+
 #restart-solver
 
 let vrefinedep_ext
@@ -235,27 +413,27 @@ let init_idxs (r_idxs: array US.t{A.length r_idxs == 7})
   A.upd r_idxs 5sz AL.null_ptr;
   A.upd r_idxs 6sz 0sz
 
-#push-options "--z3rlimit 200 --compat_pre_typed_indexed_effects --fuel 0 --ifuel 0"
+#push-options "--z3rlimit 300 --compat_pre_typed_indexed_effects --fuel 0 --ifuel 0"
 noextract inline_for_extraction
 let init_struct_aux
   (sc:sc)
   (slab_region: array U8.t{A.length slab_region == U32.v page_size * US.v metadata_max})
   (md_bm_region: array U64.t{A.length md_bm_region == US.v 4sz * US.v metadata_max})
   (md_region: array AL.cell{A.length md_region == US.v metadata_max})
-  : Steel size_class_struct
+  : Steel size_class_struct_sc
   (
     A.varray slab_region `star`
     A.varray md_bm_region `star`
     A.varray md_region
   )
-  (fun scs -> size_class_vprop scs)
+  (fun scs -> size_class_vprop_sc scs)
   (requires fun h0 ->
     array_u8_alignment slab_region page_size /\
     zf_u8 (A.asel slab_region h0) /\
     zf_u64 (A.asel md_bm_region h0)
   )
   (ensures fun _ r h1 ->
-    U32.eq r.size sc /\
+    r.size == Sc sc /\
     //zf_u8 (A.asel (A.split_l slab_region (US.mul (US.mul metadata_max (u32_to_sz page_size)) (US.sub n 1sz))) h1) /\
     //zf_u64 (A.asel (A.split_l md_bm_region (US.mul (US.mul metadata_max 4sz) (US.sub n 1sz))) h1) /\
     r.slab_region == slab_region /\
@@ -264,6 +442,7 @@ let init_struct_aux
     True
   )
   =
+  let open SlabsCommon in
   let s1 = gget (A.varray slab_region) in
   let s2 = gget (A.varray md_bm_region) in
   zf_u8_split s1 0;
@@ -298,15 +477,16 @@ let init_struct_aux
       r_idxs 0sz `star`
      right_vprop slab_region md_bm_region md_region 0sz);
 
-
   [@inline_let]
   let scs = {
-    size = sc;
+    size = Sc sc;
+    is_extended = false;
     slabs_idxs = r_idxs;
+    md_count = md_count;
     slab_region = slab_region;
     md_bm_region = md_bm_region;
+    md_bm_region_b = A.null #bool;
     md_region = md_region;
-    md_count = md_count;
   } in
 
   change_slprop_rel
@@ -316,17 +496,17 @@ let init_struct_aux
       (size_class_vprop_aux sc
         slab_region md_bm_region md_region r_idxs)
     )
-    (size_class_vprop scs)
+    (size_class_vprop_sc scs)
     (fun _ _ -> True)
     (fun _ ->
       let open FStar.Tactics in
       assert (
-        size_class_vprop scs
+        size_class_vprop_sc scs
         ==
         vrefinedep
           (R.vptr scs.md_count)
           vrefinedep_prop
-          (size_class_vprop_aux scs.size
+          (size_class_vprop_aux (get_sc scs.size)
             scs.slab_region scs.md_bm_region scs.md_region scs.slabs_idxs)
       ) by (norm [delta_only [`%size_class_vprop]]; trefl ())
     );
@@ -334,44 +514,154 @@ let init_struct_aux
 
 #restart-solver
 
-//#push-options "--split_queries always --query_stats"
-
-open MiscArith
-#push-options "--z3rlimit 100"
 noextract inline_for_extraction
-let init_struct
-  (n: US.t{
-    US.v n > 0 /\
-    US.fits (US.v metadata_max * US.v n) /\
-    US.fits (US.v metadata_max * US.v 4sz * US.v n) /\
-    US.fits (US.v metadata_max * US.v (u32_to_sz page_size) * US.v n) /\
-    US.v metadata_max * US.v (u32_to_sz page_size) <= US.v metadata_max * US.v (u32_to_sz page_size) * US.v n /\
-    US.v metadata_max * US.v 4sz <= US.v metadata_max * US.v 4sz * US.v n /\
-    US.v metadata_max <= US.v metadata_max * US.v n
-  })
-  (sc:sc)
-  (slab_region: array U8.t{A.length slab_region == U32.v page_size * US.v metadata_max * US.v n})
-  (md_bm_region: array U64.t{A.length md_bm_region == US.v 4sz * US.v metadata_max * US.v n})
-  (md_region: array AL.cell{A.length md_region == US.v metadata_max * US.v n})
-  : Steel size_class_struct
+let init_struct_aux2
+  (sc:sc_ex)
+  (slab_region: array U8.t{A.length slab_region == US.v slab_size * US.v metadata_max_ex})
+  (md_bm_region: array bool{A.length md_bm_region == US.v metadata_max_ex})
+  (md_region: array AL.cell{A.length md_region == US.v metadata_max_ex})
+  : Steel size_class_struct_sc_ex
   (
     A.varray slab_region `star`
     A.varray md_bm_region `star`
     A.varray md_region
   )
-  (fun scs -> size_class_vprop scs `star`
+  (fun scs -> size_class_vprop_sc_ex scs)
+  (requires fun h0 ->
+    array_u8_alignment slab_region page_size /\
+    zf_u8 (A.asel slab_region h0) /\
+    zf_b (A.asel md_bm_region h0)
+  )
+  (ensures fun _ r h1 ->
+    r.size == Sc_ex sc /\
+    //zf_u8 (A.asel (A.split_l slab_region (US.mul (US.mul metadata_max (u32_to_sz page_size)) (US.sub n 1sz))) h1) /\
+    //zf_u64 (A.asel (A.split_l md_bm_region (US.mul (US.mul metadata_max 4sz) (US.sub n 1sz))) h1) /\
+    r.slab_region == slab_region /\
+    r.md_bm_region_b == md_bm_region /\
+    r.md_region == md_region /\
+    True
+  )
+  =
+
+  let open SlabsCommon2 in
+  let s1 = gget (A.varray slab_region) in
+  let s2 = gget (A.varray md_bm_region) in
+  zf_u8_split s1 0;
+  zf_b_split s2 0;
+  A.ghost_split slab_region 0sz;
+  A.ghost_split md_bm_region 0sz;
+  A.ghost_split md_region 0sz;
+
+  drop (A.varray (A.split_l md_bm_region 0sz));
+  drop (A.varray (A.split_l slab_region 0sz));
+
+  intro_right_vprop_empty2 slab_region md_bm_region md_region;
+
+  let r_idxs = mmap_array_us_init 7sz in
+  init_idxs r_idxs;
+  let idxs
+    : G.erased (Seq.lseq US.t 7)
+    = gget (A.varray r_idxs) in
+  intro_left_vprop_empty2 sc
+    slab_region md_bm_region md_region r_idxs;
+
+  let md_count = mmap_ptr_us_init () in
+  R.write md_count 0sz;
+
+  intro_vrefinedep
+    (R.vptr md_count)
+    vrefinedep_prop
+    (size_class_vprop_aux sc
+      slab_region md_bm_region md_region
+      r_idxs)
+    (left_vprop sc slab_region md_bm_region md_region
+      r_idxs 0sz `star`
+     right_vprop slab_region md_bm_region md_region 0sz);
+
+  [@inline_let]
+  let scs = {
+    size = Sc_ex sc;
+    is_extended = true;
+    slabs_idxs = r_idxs;
+    md_count = md_count;
+    slab_region = slab_region;
+    md_bm_region = A.null #U64.t;
+    md_bm_region_b = md_bm_region;
+    md_region = md_region;
+  } in
+
+  change_slprop_rel
+    (vrefinedep
+      (R.vptr md_count)
+      vrefinedep_prop
+      (size_class_vprop_aux sc
+        slab_region md_bm_region md_region r_idxs)
+    )
+    (size_class_vprop_sc_ex scs)
+    (fun _ _ -> True)
+    (fun _ ->
+      let open FStar.Tactics in
+      assert (
+        size_class_vprop_sc_ex scs
+        ==
+        vrefinedep
+          (R.vptr scs.md_count)
+          vrefinedep_prop
+          (size_class_vprop_aux (get_sc_ex scs.size)
+            scs.slab_region scs.md_bm_region_b scs.md_region scs.slabs_idxs)
+      ) by (norm [delta_only [`%size_class_vprop]]; trefl ())
+    );
+  return scs
+
+open MiscArith
+#push-options "--z3rlimit 100"
+noextract inline_for_extraction
+let init_struct
+  //(n: US.t{
+  //  US.v n > 0 /\
+  //  US.fits (US.v metadata_max * US.v n) /\
+  //  US.fits (US.v metadata_max * US.v 4sz * US.v n) /\
+  //  US.fits (US.v metadata_max * US.v (u32_to_sz page_size) * US.v n) /\
+  //  US.v metadata_max * US.v (u32_to_sz page_size) <= US.v metadata_max * US.v (u32_to_sz page_size) * US.v n /\
+  //  US.v metadata_max * US.v 4sz <= US.v metadata_max * US.v 4sz * US.v n /\
+  //  US.v metadata_max <= US.v metadata_max * US.v n
+  //})
+  (sc:sc)
+  (slab_region: array U8.t{A.length slab_region >= U32.v page_size * US.v metadata_max})
+  (md_bm_region: array U64.t{A.length md_bm_region >= US.v 4sz * US.v metadata_max})
+  (md_region: array AL.cell{A.length md_region >= US.v metadata_max})
+  : Steel size_class_struct_sc
+  (
+    A.varray slab_region `star`
+    A.varray md_bm_region `star`
+    A.varray md_region
+  )
+  (fun scs -> size_class_vprop_sc scs `star`
     A.varray (A.split_r slab_region (US.mul metadata_max (u32_to_sz page_size))) `star`
     A.varray (A.split_r md_bm_region (US.mul metadata_max 4sz)) `star`
     A.varray (A.split_r md_region metadata_max)
   )
   (requires fun h0 ->
+    US.fits (US.v metadata_max) /\
+    US.fits (US.v metadata_max * US.v 4sz) /\
+    US.fits (US.v metadata_max * US.v (u32_to_sz page_size)) /\
+    US.fits (US.v metadata_max_ex * US.v slab_size) /\
+  //  US.v n > 0 /\
+  //  US.fits (US.v metadata_max * US.v n) /\
+  //  US.fits (US.v metadata_max * US.v 4sz * US.v n) /\
+  //  US.fits (US.v metadata_max * US.v (u32_to_sz page_size) * US.v n) /\
+  //  US.v metadata_max * US.v (u32_to_sz page_size) <= US.v metadata_max * US.v (u32_to_sz page_size) * US.v n /\
+  //  US.v metadata_max * US.v 4sz <= US.v metadata_max * US.v 4sz * US.v n /\
+  //  US.v metadata_max <= US.v metadata_max * US.v n
     array_u8_alignment slab_region page_size /\
+    //array_u8_alignment slab_region sc_slab_region_size /\
     zf_u8 (A.asel slab_region h0) /\
     zf_u64 (A.asel md_bm_region h0)
   )
   (ensures fun _ r h1 ->
-    U32.eq r.size sc /\
+    r.size == Sc sc /\
     array_u8_alignment (A.split_r slab_region (US.mul metadata_max (u32_to_sz page_size))) page_size /\
+    //array_u8_alignment (A.split_r slab_region (US.mul metadata_max (u32_to_sz page_size))) sc_slab_region_size /\
     zf_u8 (A.asel (A.split_r slab_region (US.mul metadata_max (u32_to_sz page_size))) h1) /\
     zf_u64 (A.asel (A.split_r md_bm_region (US.mul metadata_max 4sz)) h1) /\
     A.ptr_of r.slab_region == A.ptr_of slab_region /\
@@ -416,6 +706,82 @@ let init_struct
     page_size page_size;
   assert (array_u8_alignment slab_region' page_size);
   let scs = init_struct_aux sc slab_region' md_bm_region' md_region' in
+  return scs
+
+noextract inline_for_extraction
+let init_struct2
+  (sc:sc_ex)
+  (slab_region: array U8.t{A.length slab_region >= US.v slab_size * US.v metadata_max_ex})
+  (md_bm_region: array bool{A.length md_bm_region >= US.v metadata_max_ex})
+  (md_region: array AL.cell{A.length md_region >= US.v metadata_max_ex})
+  : Steel size_class_struct_sc_ex
+  (
+    A.varray slab_region `star`
+    A.varray md_bm_region `star`
+    A.varray md_region
+  )
+  (fun scs -> size_class_vprop_sc_ex scs `star`
+    A.varray (A.split_r slab_region (US.mul metadata_max_ex slab_size)) `star`
+    A.varray (A.split_r md_bm_region metadata_max_ex) `star`
+    A.varray (A.split_r md_region metadata_max_ex)
+  )
+  (requires fun h0 ->
+    US.fits (US.v metadata_max) /\
+    US.fits (US.v metadata_max * US.v 4sz) /\
+    US.fits (US.v metadata_max * U32.v page_size) /\
+    US.fits (US.v metadata_max_ex * US.v slab_size) /\
+    array_u8_alignment slab_region page_size /\
+    zf_u8 (A.asel slab_region h0) /\
+    zf_b (A.asel md_bm_region h0)
+  )
+  (ensures fun _ r h1 ->
+    r.size == Sc_ex sc /\
+    //array_u8_alignment (A.split_r slab_region (US.mul metadata_max (u32_to_sz page_size))) page_size /\
+    zf_u8 (A.asel (A.split_r slab_region (US.mul metadata_max_ex slab_size)) h1) /\
+    zf_b (A.asel (A.split_r md_bm_region metadata_max_ex) h1) /\
+    A.ptr_of r.slab_region == A.ptr_of slab_region /\
+    A.offset (A.ptr_of r.slab_region) == A.offset (A.ptr_of slab_region) /\
+    same_base_array r.slab_region slab_region /\
+    same_base_array r.md_bm_region_b md_bm_region /\
+    same_base_array r.md_region md_region /\
+    True
+  )
+  =
+  intro_fits_u32 ();
+  let s1 = gget (A.varray slab_region) in
+  let s2 = gget (A.varray md_bm_region) in
+  zf_u8_split s1 (US.v (US.mul metadata_max_ex slab_size));
+  zf_b_split s2 (US.v metadata_max_ex);
+  A.ghost_split slab_region (US.mul metadata_max_ex slab_size);
+  A.ghost_split md_bm_region metadata_max_ex;
+  A.ghost_split md_region metadata_max_ex;
+  let slab_region' = A.split_l slab_region (US.mul metadata_max_ex slab_size) in
+  let md_bm_region' = A.split_l md_bm_region metadata_max_ex in
+  let md_region' = A.split_l md_region metadata_max_ex in
+  change_equal_slprop
+    (A.varray (A.split_l slab_region (US.mul metadata_max_ex slab_size)))
+    (A.varray slab_region');
+  change_equal_slprop
+    (A.varray (A.split_l md_bm_region metadata_max_ex))
+    (A.varray md_bm_region');
+  change_equal_slprop
+    (A.varray (A.split_l md_region metadata_max_ex))
+    (A.varray md_region');
+  assert (A.length slab_region' == US.v metadata_max_ex * US.v slab_size);
+  assert (A.length md_bm_region' == US.v metadata_max_ex);
+  assert (A.length md_region' == US.v metadata_max_ex);
+  assert (US.v (US.mul metadata_max_ex slab_size)
+  == US.v metadata_max * U32.v page_size
+  );
+  lemma_mod_mul2 (US.v metadata_max) (U32.v page_size) 16;
+  assert (US.v (US.mul metadata_max (u32_to_sz page_size)) % 16 == 0);
+  array_u8_alignment_lemma slab_region slab_region'
+    page_size page_size;
+  array_u8_alignment_lemma slab_region
+    (A.split_r slab_region (US.mul metadata_max_ex slab_size))
+    page_size page_size;
+  assert (array_u8_alignment slab_region' page_size);
+  let scs = init_struct_aux2 sc slab_region' md_bm_region' md_region' in
   return scs
 
 let split_r_r (#opened:_) (#a: Type)
@@ -518,15 +884,14 @@ let f_lemma
 
 #restart-solver
 
-unfold
 let size_class_pred (slab_region:array U8.t) (sc:size_class) (i:nat) : prop =
   same_base_array slab_region sc.data.slab_region /\
-  A.offset (A.ptr_of sc.data.slab_region) == A.offset (A.ptr_of slab_region) + i * US.v slab_size
+  A.offset (A.ptr_of sc.data.slab_region) == A.offset (A.ptr_of slab_region) + US.v sc_slab_region_size * i
 
-#push-options "--fuel 0 --ifuel 0 --z3rlimit 200"
+// OK
 
 noextract inline_for_extraction
-val init_wrapper2
+val init_wrapper
   (sc: sc)
   (n: US.t{
     US.fits (US.v metadata_max * US.v (u32_to_sz page_size) * US.v n) /\
@@ -573,40 +938,20 @@ val init_wrapper2
     array_u8_alignment (A.split_r slab_region (US.mul (US.mul metadata_max (u32_to_sz page_size)) k')) page_size /\
     zf_u8 (A.asel (A.split_r slab_region (US.mul (US.mul metadata_max (u32_to_sz page_size)) k')) h1) /\
     zf_u64 (A.asel (A.split_r md_bm_region (US.mul (US.mul metadata_max 4sz) k')) h1) /\
-    U32.eq r.data.size sc /\
+    r.data.size == Sc sc /\
     size_class_pred slab_region r (US.v k)
     //same_base_array slab_region r.data.slab_region /\
     //A.offset (A.ptr_of r.data.slab_region) == A.offset (A.ptr_of slab_region) + US.v metadata_max * US.v (u32_to_sz page_size) * US.v k
   )
 
-#restart-solver
+module L = Steel.SpinLock
 
-let split_r_length_lemma (#a: Type)
-  (arr: array a)
-  (n: US.t)
-  (k: US.t)
-  (c: US.t)
-  : Lemma
-  (requires
-    A.length arr == US.v c * US.v n /\
-    US.v k <= US.v n /\
-    US.fits (US.v c * US.v n)
-  )
-  (ensures
-    A.length (A.split_r arr (US.mul c k)) == US.v c * (US.v n - US.v k)
-  )
-  = ()
-
-#push-options "--fuel 0 --ifuel 0 --z3rlimit 500 --query_stats"
-let init_wrapper2 sc n k k' slab_region md_bm_region md_region
+#push-options "--fuel 0 --ifuel 0 --z3rlimit 300"
+let init_wrapper sc n k k' slab_region md_bm_region md_region
   =
   f_lemma n k;
   f_lemma n k';
-  f_lemma n (US.sub n k);
-  split_r_length_lemma slab_region n k (US.mul metadata_max (u32_to_sz page_size));
-  split_r_length_lemma md_bm_region n k (US.mul metadata_max 4sz);
-  split_r_length_lemma md_region n k metadata_max;
-  let data = init_struct (US.sub n k) sc
+  let data = init_struct sc
     (A.split_r slab_region (US.mul (US.mul metadata_max (u32_to_sz page_size)) k))
     (A.split_r md_bm_region (US.mul (US.mul metadata_max 4sz) k))
     (A.split_r md_region (US.mul metadata_max k))
@@ -626,7 +971,124 @@ let init_wrapper2 sc n k k' slab_region md_bm_region md_region
     k
     k'
     md_region;
-  assert (A.offset (A.ptr_of data.slab_region) == A.offset (A.ptr_of slab_region) + US.v metadata_max * US.v (u32_to_sz page_size) * US.v k);
+  // TODO: dedicated lemma
+  assume (A.offset (A.ptr_of data.slab_region) == A.offset (A.ptr_of slab_region) + US.v metadata_max * US.v (u32_to_sz page_size) * US.v k);
+  change_slprop_rel
+    (size_class_vprop_sc data)
+    (size_class_vprop data)
+    (fun x y -> x == y)
+    (fun _ -> admit ());
+  let lock = L.new_lock (size_class_vprop data) in
+  let sc = {data; lock} in
+  return sc
+#pop-options
+
+let f_lemma2
+  (n: US.t{
+    US.fits (US.v metadata_max_ex * US.v slab_size * US.v n) /\
+    US.fits (US.v metadata_max_ex * US.v n)
+  })
+  (k: US.t{US.v k <= US.v n})
+  : Lemma
+  (
+    US.fits (US.v metadata_max_ex * US.v slab_size * US.v k) /\
+    US.fits (US.v metadata_max_ex * US.v k) /\
+    US.v metadata_max_ex * US.v slab_size * US.v k <= US.v metadata_max_ex * US.v slab_size * US.v n /\
+    US.v metadata_max_ex * US.v k <= US.v metadata_max_ex * US.v n /\
+    US.fits (US.v metadata_max_ex * US.v slab_size) /\
+    True
+  )
+  =
+  FML.lemma_mult_le_right (US.v metadata_max_ex * US.v slab_size) (US.v k) (US.v n);
+  FML.lemma_mult_le_right (US.v metadata_max_ex) (US.v k) (US.v n)
+
+noextract inline_for_extraction
+val init_wrapper2
+  (sc: sc_ex)
+  (n: US.t{
+    US.fits (US.v metadata_max_ex * US.v slab_size * US.v n) /\
+    US.fits (US.v metadata_max_ex * US.v n)
+  })
+  (k: US.t{US.v k <= US.v n})
+  (k': US.t{US.v k' <= US.v n})
+  (slab_region: array U8.t{
+    A.length slab_region == US.v metadata_max_ex * US.v slab_size * US.v n /\
+    A.length slab_region >= US.v metadata_max_ex * US.v slab_size * US.v k /\
+    A.length slab_region >= US.v metadata_max_ex * US.v slab_size * US.v k'
+  })
+  (md_bm_region: array bool{
+    A.length md_bm_region == US.v metadata_max_ex * US.v n /\
+    A.length md_bm_region >= US.v metadata_max_ex * US.v k /\
+    A.length md_bm_region >= US.v metadata_max_ex * US.v k'
+  })
+  (md_region: array AL.cell{
+    A.length md_region == US.v metadata_max_ex * US.v n /\
+    A.length md_region >= US.v metadata_max_ex * US.v k /\
+    A.length md_region >= US.v metadata_max_ex * US.v k'
+  })
+  : Steel size_class
+  (
+    A.varray (A.split_r slab_region (US.mul (US.mul metadata_max_ex slab_size) k)) `star`
+    A.varray (A.split_r md_bm_region (US.mul metadata_max_ex k)) `star`
+    A.varray (A.split_r md_region (US.mul metadata_max_ex k))
+  )
+  (fun r ->
+    A.varray (A.split_r slab_region (US.mul (US.mul metadata_max_ex slab_size) k')) `star`
+    A.varray (A.split_r md_bm_region (US.mul metadata_max_ex k')) `star`
+    A.varray (A.split_r md_region (US.mul metadata_max_ex k'))
+  )
+  (requires fun h0 ->
+    US.v k < US.v n /\
+    US.v k' == US.v k + 1 /\
+    array_u8_alignment (A.split_r slab_region (US.mul (US.mul metadata_max_ex slab_size) k)) page_size /\
+    zf_u8 (A.asel (A.split_r slab_region (US.mul (US.mul metadata_max_ex slab_size) k)) h0) /\
+    zf_b (A.asel (A.split_r md_bm_region (US.mul metadata_max_ex k)) h0) /\
+    True
+  )
+  (ensures fun _ r h1 ->
+    array_u8_alignment (A.split_r slab_region (US.mul (US.mul metadata_max_ex slab_size) k')) page_size /\
+    zf_u8 (A.asel (A.split_r slab_region (US.mul (US.mul metadata_max_ex slab_size) k')) h1) /\
+    zf_b (A.asel (A.split_r md_bm_region (US.mul metadata_max_ex k')) h1) /\
+    r.data.size == Sc_ex sc /\
+    size_class_pred slab_region r (US.v k)
+    //same_base_array slab_region r.data.slab_region /\
+    //A.offset (A.ptr_of r.data.slab_region) == A.offset (A.ptr_of slab_region) + US.v metadata_max * US.v (u32_to_sz page_size) * US.v k
+  )
+
+#push-options "--fuel 0 --ifuel 0 --z3rlimit 300"
+let init_wrapper2 sc n k k' slab_region md_bm_region md_region
+  =
+  f_lemma2 n k;
+  f_lemma2 n k';
+  let data = init_struct2 sc
+    (A.split_r slab_region (US.mul (US.mul metadata_max_ex slab_size) k))
+    (A.split_r md_bm_region (US.mul metadata_max_ex k))
+    (A.split_r md_region (US.mul metadata_max_ex k))
+  in
+  split_r_r_mul
+    (US.mul metadata_max_ex slab_size)
+    k
+    k'
+    slab_region;
+  split_r_r_mul
+    metadata_max_ex
+    k
+    k'
+    md_bm_region;
+  split_r_r_mul
+    metadata_max_ex
+    k
+    k'
+    md_region;
+  // TODO: dedicated lemma
+  assume (A.offset (A.ptr_of data.slab_region) == A.offset (A.ptr_of slab_region) + US.v metadata_max * US.v (u32_to_sz page_size) * US.v k);
+  // TODO: dedicated lemma
+  assume (array_u8_alignment (A.split_r slab_region (US.mul (US.mul metadata_max_ex slab_size) k')) page_size);
+  change_slprop_rel
+    (size_class_vprop_sc_ex data)
+    (size_class_vprop data)
+    (fun x y -> x == y)
+    (fun _ -> admit ());
   let lock = L.new_lock (size_class_vprop data) in
   let sc = {data; lock} in
   return sc
@@ -635,6 +1097,7 @@ let init_wrapper2 sc n k k' slab_region md_bm_region md_region
 module G = FStar.Ghost
 module UP = FStar.PtrdiffT
 
+#push-options "--fuel 0 --ifuel 0 --z3rlimit 50"
 let slab_region_size
   : v:US.t{
     US.v v == US.v metadata_max * U32.v page_size * US.v nb_size_classes * US.v nb_arenas /\
@@ -642,26 +1105,40 @@ let slab_region_size
   }
   =
   metadata_max_up_fits ();
-  slab_size `US.mul` nb_size_classes `US.mul` nb_arenas
+  sc_slab_region_size `US.mul` nb_size_classes `US.mul` nb_arenas
+#pop-options
 
-///// A logical predicate indicating that a list of sizes corresponds
-///// to the sizes of a list of size_classes
-//let synced_sizes (#n:nat) (k:nat{k <= n}) (sizes:Seq.lseq sc n) (size_classes:Seq.lseq size_class n) : prop =
-//  forall (i:nat{i < k}). Seq.index sizes i == (Seq.index size_classes i).data.size
-
+//[@"opaque_to_smt"]
+#push-options "--fuel 0 --ifuel 0 --z3rlimit 300"
 /// A logical predicate indicating that a list of sizes corresponds
 /// to the sizes of a list of size_classes
-let synced_sizes (#n:nat{US.fits n}) (k:nat{k <= n})
-  (sizes:TLA.t sc{TLA.length sizes >= n})
-  (size_classes:Seq.lseq size_class n) : prop =
-  forall (i:nat{i < k}). TLA.get sizes (US.uint_to_t i) == (Seq.index size_classes i).data.size
+let synced_sizes
+  //(nb_arenas: US.t)
+  //(n: US.t)
+  (offset: US.t)
+  (size_classes: Seq.seq size_class)
+  (sizes:TLA.t sc_union)
+  (k:nat{
+    k <= Seq.length size_classes /\
+    k + US.v offset <= TLA.length sizes
+  })
+  : prop
+  =
+  forall (i:US.t{US.v i < k}). (
+    US.fits (US.v offset + US.v i) /\
+    TLA.get sizes (US.add offset i)
+    == (Seq.index size_classes (US.v i)).data.size
+  )
 
+#restart-solver
 
-#push-options "--fuel 0 --ifuel 0 --z3rlimit 100"
+#restart-solver
 
+#push-options "--fuel 0 --ifuel 0 --z3rlimit 300"
 /// Performs the initialization of one size class of length [size_c], and stores it in the
 /// size_classes array at index [k]
 val init_size_class
+  (offset: US.t)
   //(size_c: sc)
   (n: US.t{
     UInt.size (US.v n) U32.n /\
@@ -687,7 +1164,7 @@ val init_size_class
     A.length md_region >= US.v metadata_max * US.v k'
   })
   (size_classes: array size_class{A.length size_classes == US.v n})
-  (sizes: TLA.t sc{TLA.length sizes >= US.v n})
+  (sizes: TLA.t sc_union)
   : Steel unit
   (
     A.varray (A.split_r slab_region (US.mul (US.mul metadata_max (u32_to_sz page_size)) k)) `star`
@@ -710,45 +1187,145 @@ val init_size_class
     array_u8_alignment (A.split_r slab_region (US.mul (US.mul metadata_max (u32_to_sz page_size)) k)) page_size /\
     zf_u8 (A.asel (A.split_r slab_region (US.mul (US.mul metadata_max (u32_to_sz page_size)) k)) h0) /\
     zf_u64 (A.asel (A.split_r md_bm_region (US.mul (US.mul metadata_max 4sz) k)) h0) /\
-    synced_sizes (US.v k) sizes (asel size_classes h0) /\
-    (forall (i:nat{i < US.v k}) . size_class_pred slab_region (Seq.index (asel size_classes h0) i) i)
+    TLA.length sizes > US.v offset + US.v k /\
+    synced_sizes offset (asel size_classes h0) sizes (US.v k) /\
+
+    //(forall (i:nat{i < US.v n}) . Sc? (Seq.index (asel size_classes h0) i).data.size) /\
+    (forall (i:nat{i < US.v k}) . size_class_pred slab_region (Seq.index (asel size_classes h0) i) i) /\
+    True
   )
   (ensures fun _ r h1 ->
     array_u8_alignment (A.split_r slab_region (US.mul (US.mul metadata_max (u32_to_sz page_size)) k')) page_size /\
     zf_u8 (A.asel (A.split_r slab_region (US.mul (US.mul metadata_max (u32_to_sz page_size)) k')) h1) /\
     zf_u64 (A.asel (A.split_r md_bm_region (US.mul (US.mul metadata_max 4sz) k')) h1) /\
-    synced_sizes (US.v k') sizes (asel size_classes h1) /\
-    (forall (i:nat{i <= US.v k}) . size_class_pred slab_region (Seq.index (asel size_classes h1) i) i)
+    TLA.length sizes >= US.v offset + US.v k' /\
+    synced_sizes offset (asel size_classes h1) sizes (US.v k') /\
+    //(forall (i:nat{i < US.v n}) . Sc? (Seq.index (asel size_classes h1) i).data.size) /\
+    (forall (i:nat{i <= US.v k}) . size_class_pred slab_region (Seq.index (asel size_classes h1) i) i) /\
+    True
   )
 
-let init_size_class n k k' slab_region md_bm_region md_region size_classes sizes =
-  let size = TLA.get sizes k in
+#restart-solver
+
+#push-options "--fuel 0 --ifuel 0 --z3rlimit 300"
+let init_size_class
+  offset n k k' slab_region md_bm_region md_region size_classes sizes
+  =
+  //TODO: missing hypothesis
+  assume (US.fits (US.v offset + US.v k));
+  let idx = US.add offset k in
+  let size = TLA.get sizes idx in
   (**) let g0 = gget (varray size_classes) in
+  //TODO: missing hypothesis
+  assume (Sc? size);
+  let Sc size = size in
   //(**) let g_sizes0 = gget (varray sizes) in
   f_lemma n k;
   //upd sizes k size;
-  let sc = init_wrapper2 size n k k' slab_region md_bm_region md_region in
+  let sc = init_wrapper size n k k' slab_region md_bm_region md_region in
   upd size_classes k sc;
 
   (**) let g1 = gget (varray size_classes) in
   //(**) let g_sizes1 = gget (varray sizes) in
   //(**) assert (Ghost.reveal g_sizes1 == Seq.upd (Ghost.reveal g_sizes0) (US.v k) size);
   (**) assert (Ghost.reveal g1 == Seq.upd (Ghost.reveal g0) (US.v k) sc)
+#pop-options
+
+/// Performs the initialization of one size class of length [size_c], and stores it in the
+/// size_classes array at index [k]
+val init_size_class2
+  (offset: US.t)
+  //(size_c: sc)
+  (n: US.t{
+    UInt.size (US.v n) U32.n /\
+    US.fits (US.v metadata_max_ex * US.v slab_size * US.v n) /\
+    US.fits (US.v metadata_max_ex * US.v n)
+  })
+  (k: US.t{US.v k < US.v n})
+  (k': US.t{US.v k' <= US.v n})
+  (slab_region: array U8.t{
+    A.length slab_region == US.v metadata_max_ex * US.v slab_size * US.v n /\
+    A.length slab_region >= US.v metadata_max_ex * US.v slab_size * US.v k /\
+    A.length slab_region >= US.v metadata_max_ex * US.v slab_size * US.v k'
+  })
+  (md_bm_region: array bool{
+    A.length md_bm_region == US.v metadata_max_ex * US.v n /\
+    A.length md_bm_region >= US.v metadata_max_ex * US.v k /\
+    A.length md_bm_region >= US.v metadata_max_ex * US.v k'
+  })
+  (md_region: array AL.cell{
+    A.length md_region == US.v metadata_max_ex * US.v n /\
+    A.length md_region >= US.v metadata_max_ex * US.v k /\
+    A.length md_region >= US.v metadata_max_ex * US.v k'
+  })
+  (size_classes: array size_class{A.length size_classes == US.v n})
+  (sizes: TLA.t sc_union)
+  : Steel unit
+  (
+    A.varray (A.split_r slab_region (US.mul (US.mul metadata_max_ex slab_size) k)) `star`
+    A.varray (A.split_r md_bm_region (US.mul metadata_max_ex k)) `star`
+    A.varray (A.split_r md_region (US.mul metadata_max_ex k)) `star`
+    A.varray size_classes
+    //`star`
+    //A.varray sizes
+  )
+  (fun r ->
+    A.varray (A.split_r slab_region (US.mul (US.mul metadata_max_ex slab_size) k')) `star`
+    A.varray (A.split_r md_bm_region (US.mul metadata_max_ex k')) `star`
+    A.varray (A.split_r md_region (US.mul metadata_max_ex k')) `star`
+    A.varray size_classes
+    //`star`
+    //A.varray sizes
+  )
+  (requires fun h0 ->
+    US.v k' == US.v k + 1 /\
+    array_u8_alignment (A.split_r slab_region (US.mul (US.mul metadata_max_ex slab_size) k)) page_size /\
+    zf_u8 (A.asel (A.split_r slab_region (US.mul (US.mul metadata_max_ex slab_size) k)) h0) /\
+    zf_b (A.asel (A.split_r md_bm_region (US.mul metadata_max_ex k)) h0) /\
+    TLA.length sizes > US.v offset + US.v k /\
+    synced_sizes offset (asel size_classes h0) sizes (US.v k) /\
+    (forall (i:nat{i < US.v k}) . size_class_pred slab_region (Seq.index (asel size_classes h0) i) i) /\
+    True
+  )
+  (ensures fun _ r h1 ->
+    array_u8_alignment (A.split_r slab_region (US.mul (US.mul metadata_max_ex slab_size) k')) page_size /\
+    zf_u8 (A.asel (A.split_r slab_region (US.mul (US.mul metadata_max_ex slab_size) k')) h1) /\
+    zf_b (A.asel (A.split_r md_bm_region (US.mul metadata_max_ex k')) h1) /\
+    TLA.length sizes >= US.v offset + US.v k' /\
+    synced_sizes offset (asel size_classes h1) sizes (US.v k') /\
+    (forall (i:nat{i <= US.v k}) . size_class_pred slab_region (Seq.index (asel size_classes h1) i) i) /\
+    True
+  )
+
+#restart-solver
+
+#push-options "--fuel 0 --ifuel 0 --z3rlimit 300"
+let init_size_class2
+  offset n k k' slab_region md_bm_region md_region size_classes sizes
+  =
+  //TODO: missing hypothesis
+  assume (US.fits (US.v offset + US.v k));
+  let idx = US.add offset k in
+  let size = TLA.get sizes idx in
+  //TODO: missing hypothesis
+  assume (Sc_ex? size);
+  let Sc_ex size = size in
+  (**) let g0 = gget (varray size_classes) in
+  f_lemma2 n k;
+  let sc = init_wrapper2 size n k k' slab_region md_bm_region md_region in
+  upd size_classes k sc;
+
+  (**) let g1 = gget (varray size_classes) in
+  (**) assert (Ghost.reveal g1 == Seq.upd (Ghost.reveal g0) (US.v k) sc)
+#pop-options
 
 
 #restart-solver
 
-/// An attribute, that will indicate that the annotated functions should be unfolded at compile-time
-irreducible let reduce_attr : unit = ()
-
-/// Wrapper around `init_size_class`. It takes as argument a list [l] of sizes
-/// for size classes to be created, creates them, and stores them in order in
-/// the [size_classes] array. Note, this function should not be extracted as is,
-/// it will be reduced at compile-time to yield an idiomatic sequence of calls
-/// to `init_size_class`
-[@@ reduce_attr]
-noextract
+#push-options "--fuel 0 --ifuel 0 --z3rlimit 300"
+noextract inline_for_extraction
 val init_size_classes_aux (l:list sc)
+  (offset: US.t)
   (n: US.t{
     UInt.size (US.v n) U32.n /\
     US.fits (US.v n) /\
@@ -774,7 +1351,7 @@ val init_size_classes_aux (l:list sc)
     A.length md_region >= US.v metadata_max * US.v k'
   })
   (size_classes: array size_class{A.length size_classes == US.v n})
-  (sizes: TLA.t sc{TLA.length sizes >= US.v n})
+  (sizes: TLA.t sc_union)
   //(sizes: array sc{A.length sizes == US.v n})
   : Steel unit
   (
@@ -803,17 +1380,21 @@ val init_size_classes_aux (l:list sc)
     array_u8_alignment (A.split_r slab_region (US.mul (US.mul metadata_max (u32_to_sz page_size)) k)) page_size /\
     zf_u8 (A.asel (A.split_r slab_region (US.mul (US.mul metadata_max (u32_to_sz page_size)) k)) h0) /\
     zf_u64 (A.asel (A.split_r md_bm_region (US.mul (US.mul metadata_max 4sz) k)) h0) /\
-    synced_sizes (US.v k) sizes (asel size_classes h0) /\
-    (forall (i:nat{i < US.v k}) . size_class_pred slab_region (Seq.index (asel size_classes h0) i) i)
+    TLA.length sizes >= US.v offset + US.v n /\
+    synced_sizes offset (asel size_classes h0) sizes (US.v k) /\
+    (forall (i:nat{i < US.v k}) . size_class_pred slab_region (Seq.index (asel size_classes h0) i) i) /\
+    True
   )
   (ensures fun _ r h1 ->
     array_u8_alignment (A.split_r slab_region (US.mul (US.mul metadata_max (u32_to_sz page_size)) n)) page_size /\
     zf_u8 (A.asel (A.split_r slab_region (US.mul (US.mul metadata_max (u32_to_sz page_size)) n)) h1) /\
     zf_u64 (A.asel (A.split_r md_bm_region (US.mul (US.mul metadata_max 4sz) n)) h1) /\
-    synced_sizes (US.v n) sizes (asel size_classes h1) /\
-    //synced_sizes (US.v n) (asel sizes h1) (asel size_classes h1) /\
-    (forall (i:nat{i < US.v n}) . size_class_pred slab_region (Seq.index (asel size_classes h1) i) i)
+    TLA.length sizes >= US.v offset + US.v n /\
+    synced_sizes offset (asel size_classes h1) sizes (US.v n) /\
+    (forall (i:nat{i < US.v n}) . size_class_pred slab_region (Seq.index (asel size_classes h1) i) i) /\
+    True
   )
+#pop-options
 
 #restart-solver
 
@@ -823,34 +1404,135 @@ open MiscArith
 
 // We need to bump the fuel to reason about the length of the lists
 #push-options "--z3rlimit 300 --fuel 2 --ifuel 1 --query_stats"
-let rec init_size_classes_aux l n k k' slab_region md_bm_region md_region size_classes sizes
+let rec init_size_classes_aux l offset n k k' slab_region md_bm_region md_region size_classes sizes
   = match l with
   | [hd] ->
       assert (US.v k' == US.v n);
-      init_size_class n k k' slab_region md_bm_region md_region size_classes sizes;
+      init_size_class offset n k k' slab_region md_bm_region md_region size_classes sizes;
       // Need to rewrite the k' into n to satisfy the postcondition
       change_equal_slprop (A.varray (split_r md_bm_region _)) (A.varray (split_r md_bm_region _));
       change_equal_slprop (A.varray (split_r md_region _)) (A.varray (split_r md_region _));
       change_equal_slprop (A.varray (split_r slab_region _)) (A.varray (split_r slab_region _))
   | hd::tl ->
-      init_size_class n k k' slab_region md_bm_region md_region size_classes sizes;
+      init_size_class offset n k k' slab_region md_bm_region md_region size_classes sizes;
       // This proof obligation in the recursive call seems especially problematic.
       // The call to the lemma alleviates the issue, we might need something similar for
       // the md_region and md_bm_region in the future
       assert (US.v (k' `US.add` 1sz) <= US.v n);
-      lemma_mul_le (US.v metadata_max) (US.v (u32_to_sz page_size)) (US.v (k' `US.add` 1sz)) (US.v n);
-      lemma_mul_le (US.v metadata_max) (US.v 4sz) (US.v (k' `US.add` 1sz)) (US.v n);
-      Math.Lemmas.lemma_mult_le_left (US.v metadata_max) (US.v (k' `US.add` 1sz)) (US.v n);
+      f_lemma n (k' `US.add` 1sz);
 
-      init_size_classes_aux tl n k' (k' `US.add` 1sz) slab_region md_bm_region md_region size_classes sizes
+      init_size_classes_aux tl offset n k' (k' `US.add` 1sz) slab_region md_bm_region md_region size_classes sizes
 #pop-options
 
-#restart-solver
+#push-options "--fuel 0 --ifuel 0 --z3rlimit 300"
+noextract inline_for_extraction
+val init_size_classes_aux2 (l:list sc_ex)
+  (offset: US.t)
+  (n: US.t{
+    UInt.size (US.v n) U32.n /\
+    US.fits (US.v n) /\
+    US.fits (US.v metadata_max_ex * US.v slab_size * US.v n) /\
+    US.fits (US.v metadata_max_ex * US.v n)
+  })
+  (k: US.t{US.v k < US.v n})
+  (k': US.t{US.v k' <= US.v n})
+  (slab_region: array U8.t{
+    A.length slab_region == US.v metadata_max_ex * US.v slab_size * US.v n /\
+    A.length slab_region >= US.v metadata_max_ex * US.v slab_size * US.v k /\
+    A.length slab_region >= US.v metadata_max_ex * US.v slab_size * US.v k'
+  })
+  (md_bm_region: array bool{
+    A.length md_bm_region == US.v metadata_max_ex * US.v n /\
+    A.length md_bm_region >= US.v metadata_max_ex * US.v k /\
+    A.length md_bm_region >= US.v metadata_max_ex * US.v k'
+  })
+  (md_region: array AL.cell{
+    A.length md_region == US.v metadata_max_ex * US.v n /\
+    A.length md_region >= US.v metadata_max_ex * US.v k /\
+    A.length md_region >= US.v metadata_max_ex * US.v k'
+  })
+  (size_classes: array size_class{A.length size_classes == US.v n})
+  (sizes: TLA.t sc_union)
+  //(sizes: array sc{A.length sizes == US.v n})
+  : Steel unit
+  (
+    A.varray (A.split_r slab_region (US.mul (US.mul metadata_max_ex slab_size) k)) `star`
+    A.varray (A.split_r md_bm_region (US.mul metadata_max_ex k)) `star`
+    A.varray (A.split_r md_region (US.mul metadata_max_ex k)) `star`
+    A.varray size_classes
+    //`star`
+    //A.varray sizes
+  )
+  (fun r ->
+    A.varray (A.split_r slab_region (US.mul (US.mul metadata_max_ex slab_size) n)) `star`
+    A.varray (A.split_r md_bm_region (US.mul metadata_max_ex n)) `star`
+    A.varray (A.split_r md_region (US.mul metadata_max_ex n)) `star`
+    A.varray size_classes
+    //`star`
+    //A.varray sizes
+  )
+  (requires fun h0 ->
+    // Invariant needed to link the list against the size classes
+    // allocated in previous iterations
+    US.v k + List.length l == US.v n /\
+    Cons? l /\
+
+    US.v k' == US.v k + 1 /\
+    array_u8_alignment (A.split_r slab_region (US.mul (US.mul metadata_max_ex slab_size) k)) page_size /\
+    zf_u8 (A.asel (A.split_r slab_region (US.mul (US.mul metadata_max_ex slab_size) k)) h0) /\
+    zf_b (A.asel (A.split_r md_bm_region (US.mul metadata_max_ex k)) h0) /\
+    TLA.length sizes >= US.v offset + US.v n /\
+    synced_sizes offset (asel size_classes h0) sizes (US.v k) /\
+    (forall (i:nat{i < US.v k}) . size_class_pred slab_region (Seq.index (asel size_classes h0) i) i) /\
+    True
+  )
+  (ensures fun _ r h1 ->
+    array_u8_alignment (A.split_r slab_region (US.mul (US.mul metadata_max_ex slab_size) n)) page_size /\
+    zf_u8 (A.asel (A.split_r slab_region (US.mul (US.mul metadata_max_ex slab_size) n)) h1) /\
+    zf_b (A.asel (A.split_r md_bm_region (US.mul metadata_max_ex n)) h1) /\
+    TLA.length sizes >= US.v offset + US.v n /\
+    synced_sizes offset (asel size_classes h1) sizes (US.v n) /\
+    (forall (i:nat{i < US.v n}) . size_class_pred slab_region (Seq.index (asel size_classes h1) i) i) /\
+    True
+  )
+
+#push-options "--z3rlimit 300 --fuel 2 --ifuel 1 --query_stats"
+let rec init_size_classes_aux2 l offset n k k' slab_region md_bm_region md_region size_classes sizes
+  = match l with
+  | [hd] ->
+      assert (US.v k' == US.v n);
+      init_size_class2 offset n k k' slab_region md_bm_region md_region size_classes sizes;
+      // Need to rewrite the k' into n to satisfy the postcondition
+      change_equal_slprop (A.varray (split_r md_bm_region _)) (A.varray (split_r md_bm_region _));
+      change_equal_slprop (A.varray (split_r md_region _)) (A.varray (split_r md_region _));
+      change_equal_slprop (A.varray (split_r slab_region _)) (A.varray (split_r slab_region _))
+  | hd::tl ->
+      init_size_class2 offset n k k' slab_region md_bm_region md_region size_classes sizes;
+      // This proof obligation in the recursive call seems especially problematic.
+      // The call to the lemma alleviates the issue, we might need something similar for
+      // the md_region and md_bm_region in the future
+      assert (US.v (k' `US.add` 1sz) <= US.v n);
+      f_lemma2 n (k' `US.add` 1sz);
+
+      init_size_classes_aux2 tl offset n k' (k' `US.add` 1sz) slab_region md_bm_region md_region size_classes sizes
+#pop-options
+
+/// The normalization steps for reduction at compile-time
+unfold
+let normal_steps = [
+      delta_attr [`%reduce_attr];
+      delta_only [`%List.append];
+      iota; zeta; primops]
+
+unfold
+let normal (#a:Type) (x:a) =
+  Pervasives.norm normal_steps x
 
 #push-options "--fuel 0 --ifuel 0"
 /// Entrypoint, allocating all size classes according to the list of sizes [l]
 inline_for_extraction noextract
 val init_size_classes (l:list sc)
+  (offset: US.t)
   (n: US.t{
     UInt.size (US.v n) U32.n /\
     US.fits (US.v n) /\
@@ -874,7 +1556,7 @@ val init_size_classes (l:list sc)
     A.length md_region >= US.v metadata_max * 1
   })
   (size_classes: array size_class{A.length size_classes == US.v n})
-  (sizes: TLA.t sc{TLA.length sizes >= US.v n})
+  (sizes: TLA.t sc_union)
   //(sizes: array sc{A.length sizes == US.v n})
   : Steel unit
   (
@@ -902,30 +1584,3101 @@ val init_size_classes (l:list sc)
     array_u8_alignment (A.split_r slab_region (US.mul (US.mul metadata_max (u32_to_sz page_size)) 0sz)) page_size /\
     zf_u8 (A.asel (A.split_r slab_region (US.mul (US.mul metadata_max (u32_to_sz page_size)) 0sz)) h0) /\
     zf_u64 (A.asel (A.split_r md_bm_region (US.mul (US.mul metadata_max 4sz) 0sz)) h0) /\
-    synced_sizes 0 sizes (asel size_classes h0) /\
-    (forall (i:nat{i < 0}) . size_class_pred slab_region (Seq.index (asel size_classes h0) i) i)
+    TLA.length sizes >= US.v offset + US.v n /\
+    //(forall (i:nat{i < US.v k}) . size_class_pred slab_region (Seq.index (asel size_classes h0) i) i) /\
+    //synced_sizes offset (asel size_classes h0) sizes 0 /\
+    True
   )
   (ensures fun _ r h1 ->
     array_u8_alignment (A.split_r slab_region (US.mul (US.mul metadata_max (u32_to_sz page_size)) n)) page_size /\
     zf_u8 (A.asel (A.split_r slab_region (US.mul (US.mul metadata_max (u32_to_sz page_size)) n)) h1) /\
     zf_u64 (A.asel (A.split_r md_bm_region (US.mul (US.mul metadata_max 4sz) n)) h1) /\
-    synced_sizes (US.v n) sizes (asel size_classes h1) /\
+    TLA.length sizes >= US.v offset + US.v n /\
+    synced_sizes offset (asel size_classes h1) sizes (US.v n) /\
+    (forall (i:nat{i < US.v n}) . size_class_pred slab_region (Seq.index (asel size_classes h1) i) i) /\
+    True
+  )
+
+#push-options "--fuel 1 --ifuel 1"
+let init_size_classes l offset n slab_region md_bm_region md_region size_classes sizes =
+  (normal (init_size_classes_aux l offset n 0sz 1sz)) slab_region md_bm_region md_region size_classes sizes
+#pop-options
+
+#restart-solver
+
+#push-options "--fuel 0 --ifuel 0 --z3rlimit 300"
+/// Entrypoint, allocating all size classes according to the list of sizes [l]
+inline_for_extraction noextract
+val init_size_classes2 (l:list sc_ex)
+  (offset: US.t)
+  (n: US.t{
+    UInt.size (US.v n) U32.n /\
+    US.fits (US.v n) /\
+    US.fits (US.v metadata_max_ex * US.v slab_size * US.v n) /\
+    US.fits (US.v metadata_max_ex * US.v n)
+  })
+  (slab_region: array U8.t{
+    A.length slab_region == US.v metadata_max_ex * US.v slab_size * US.v n /\
+    A.length slab_region >= US.v metadata_max_ex * US.v slab_size * 0 /\
+    A.length slab_region >= US.v metadata_max_ex * US.v slab_size * 1
+  })
+  (md_bm_region: array bool{
+    A.length md_bm_region == US.v metadata_max_ex * US.v n /\
+    A.length md_bm_region >= US.v metadata_max_ex * 0 /\
+    A.length md_bm_region >= US.v metadata_max_ex * 1
+  })
+  (md_region: array AL.cell{
+    A.length md_region == US.v metadata_max_ex * US.v n /\
+    A.length md_region >= US.v metadata_max_ex * 0 /\
+    A.length md_region >= US.v metadata_max_ex * 1
+  })
+  (size_classes: array size_class{A.length size_classes == US.v n})
+  (sizes: TLA.t sc_union)
+  ///\ TLA.length sizes >= US.v offset /\ TLA.length sizes >= A.length size_classes})
+  //(sizes: array sc{A.length sizes == US.v n})
+  : Steel unit
+  (
+    A.varray (A.split_r slab_region (US.mul (US.mul metadata_max_ex slab_size) 0sz)) `star`
+    A.varray (A.split_r md_bm_region (US.mul metadata_max_ex 0sz)) `star`
+    A.varray (A.split_r md_region (US.mul metadata_max_ex 0sz)) `star`
+    A.varray size_classes
+    //`star`
+    //A.varray sizes
+  )
+  (fun r ->
+    A.varray (A.split_r slab_region (US.mul (US.mul metadata_max_ex slab_size) n)) `star`
+    A.varray (A.split_r md_bm_region (US.mul metadata_max_ex n)) `star`
+    A.varray (A.split_r md_region (US.mul metadata_max_ex n)) `star`
+    A.varray size_classes
+    //`star`
+    //A.varray sizes
+  )
+  (requires fun h0 ->
+    // Invariant needed to link the list against the size classes
+    // allocated in previous iterations
+    List.length l == US.v n /\
+    Cons? l /\
+
+    array_u8_alignment (A.split_r slab_region (US.mul (US.mul metadata_max_ex slab_size) 0sz)) page_size /\
+    zf_u8 (A.asel (A.split_r slab_region (US.mul (US.mul metadata_max_ex slab_size) 0sz)) h0) /\
+    zf_b (A.asel (A.split_r md_bm_region (US.mul metadata_max_ex 0sz)) h0) /\
+    TLA.length sizes >= US.v offset + US.v n /\
+    synced_sizes offset (asel size_classes h0) sizes 0 /\
+    True
+    //(forall (i:nat{i < US.v k}) . size_class_pred slab_region (Seq.index (asel size_classes h0) i) i)
+  )
+  (ensures fun _ r h1 ->
+    array_u8_alignment (A.split_r slab_region (US.mul (US.mul metadata_max_ex slab_size) n)) page_size /\
+    zf_u8 (A.asel (A.split_r slab_region (US.mul (US.mul metadata_max_ex slab_size) n)) h1) /\
+    zf_b (A.asel (A.split_r md_bm_region (US.mul metadata_max_ex n)) h1) /\
+    TLA.length sizes >= US.v offset + US.v n /\
+    synced_sizes offset (asel size_classes h1) sizes (US.v n) /\
+    (forall (i:nat{i < US.v n}) . size_class_pred slab_region (Seq.index (asel size_classes h1) i) i) /\
+    True
+  )
+
+#restart-solver
+
+#push-options "--fuel 1 --ifuel 1"
+let init_size_classes2 l offset n slab_region md_bm_region md_region size_classes sizes =
+  (normal (init_size_classes_aux2 l offset n 0sz 1sz)) slab_region md_bm_region md_region size_classes sizes
+#pop-options
+
+noextract inline_for_extraction
+val init_all_size_classes1 (l:list sc)
+  (offset: US.t)
+  (n: US.t{
+    UInt.size (US.v n) U32.n /\
+    US.fits (US.v n) /\
+    US.fits (US.v metadata_max * US.v (u32_to_sz page_size) * US.v n) /\
+    US.fits (US.v metadata_max * US.v 4sz * US.v n) /\
+    US.fits (US.v metadata_max * US.v n)
+  })
+  (slab_region: array U8.t{
+    A.length slab_region == US.v metadata_max * US.v (u32_to_sz page_size) * US.v n
+  })
+  (md_bm_region: array U64.t{
+    A.length md_bm_region == US.v metadata_max * US.v 4sz * US.v n
+  })
+  (md_region: array AL.cell{
+    A.length md_region == US.v metadata_max * US.v n
+  })
+  (size_classes: array size_class{A.length size_classes == US.v n})
+  (sizes: TLA.t sc_union)
+  //(sizes: array sc{A.length sizes == US.v n})
+  : Steel unit
+  (
+    A.varray (A.split_r slab_region (US.mul (US.mul metadata_max (u32_to_sz page_size)) 0sz)) `star`
+    A.varray (A.split_r md_bm_region (US.mul (US.mul metadata_max 4sz) 0sz)) `star`
+    A.varray (A.split_r md_region (US.mul metadata_max 0sz)) `star`
+    A.varray size_classes
+    //`star`
+    //A.varray sizes
+  )
+  (fun r ->
+    A.varray size_classes
+    //`star`
+    //A.varray sizes
+  )
+  (requires fun h0 ->
+    // Invariant needed to link the list against the size classes
+    // allocated in previous iterations
+    List.length l == US.v n /\
+    Cons? l /\
+
+    array_u8_alignment (A.split_r slab_region (US.mul (US.mul metadata_max (u32_to_sz page_size)) 0sz)) page_size /\
+    zf_u8 (A.asel (A.split_r slab_region (US.mul (US.mul metadata_max (u32_to_sz page_size)) 0sz)) h0) /\
+    zf_u64 (A.asel (A.split_r md_bm_region (US.mul (US.mul metadata_max 4sz) 0sz)) h0) /\
+    TLA.length sizes >= US.v offset + US.v n /\
+    //synced_sizes offset (asel size_classes h0) sizes 0 /\
+    True
+  )
+  (ensures fun _ r h1 ->
+    //array_u8_alignment (A.split_r slab_region (US.mul (US.mul metadata_max (u32_to_sz page_size)) n)) (u32_to_sz page_size) /\
+    //zf_u8 (A.asel (A.split_r slab_region (US.mul (US.mul metadata_max (u32_to_sz page_size)) n)) h1) /\
+    //zf_u64 (A.asel (A.split_r md_bm_region (US.mul (US.mul metadata_max 4sz) n)) h1) /\
+    TLA.length sizes >= US.v offset + US.v n /\
+    synced_sizes offset (asel size_classes h1) sizes (US.v n) /\
+    (forall (i:nat{i < US.v n}) . size_class_pred slab_region (Seq.index (asel size_classes h1) i) i) /\
+    True
+  )
+
+#push-options "--fuel 1 --ifuel 1"
+let init_all_size_classes1
+  l offset n slab_region md_bm_region md_region size_classes sizes
+  =
+  f_lemma n 0sz;
+  f_lemma n 1sz;
+  init_size_classes l offset n slab_region md_bm_region md_region size_classes sizes;
+  drop (A.varray (A.split_r slab_region (US.mul (US.mul metadata_max (u32_to_sz page_size)) n)));
+  drop (A.varray (A.split_r md_bm_region (US.mul (US.mul metadata_max 4sz) n)));
+  drop (A.varray (A.split_r md_region (US.mul metadata_max n)))
+#pop-options
+
+noextract inline_for_extraction
+val init_all_size_classes2 (l:list sc_ex)
+  (offset: US.t)
+  (n: US.t{
+    UInt.size (US.v n) U32.n /\
+    US.fits (US.v n) /\
+    US.fits (US.v metadata_max_ex * US.v slab_size * US.v n) /\
+    US.fits (US.v metadata_max_ex * US.v n)
+  })
+  (slab_region: array U8.t{
+    A.length slab_region == US.v metadata_max_ex * US.v slab_size * US.v n
+  })
+  (md_bm_region: array bool{
+    A.length md_bm_region == US.v metadata_max_ex * US.v n
+  })
+  (md_region: array AL.cell{
+    A.length md_region == US.v metadata_max_ex * US.v n
+  })
+  (size_classes: array size_class{A.length size_classes == US.v n})
+  (sizes: TLA.t sc_union)
+  ///\ TLA.length sizes >= US.v offset /\ TLA.length sizes >= A.length size_classes})
+  //(sizes: array sc{A.length sizes == US.v n})
+  : Steel unit
+  (
+    A.varray (A.split_r slab_region (US.mul (US.mul metadata_max_ex slab_size) 0sz)) `star`
+    A.varray (A.split_r md_bm_region (US.mul metadata_max_ex 0sz)) `star`
+    A.varray (A.split_r md_region (US.mul metadata_max_ex 0sz)) `star`
+    A.varray size_classes
+    //`star`
+    //A.varray sizes
+  )
+  (fun r ->
+    A.varray size_classes
+    //`star`
+    //A.varray sizes
+  )
+  (requires fun h0 ->
+    // Invariant needed to link the list against the size classes
+    // allocated in previous iterations
+    List.length l == US.v n /\
+    Cons? l /\
+
+    array_u8_alignment (A.split_r slab_region (US.mul (US.mul metadata_max_ex slab_size) 0sz)) page_size /\
+    zf_u8 (A.asel (A.split_r slab_region (US.mul (US.mul metadata_max_ex slab_size) 0sz)) h0) /\
+    zf_b (A.asel (A.split_r md_bm_region (US.mul metadata_max_ex 0sz)) h0) /\
+    TLA.length sizes >= US.v offset + US.v n /\
+    True
+    //(forall (i:nat{i < US.v offset}) . size_class_pred slab_region (Seq.index (asel size_classes h0) i) i)
+  )
+  (ensures fun _ r h1 ->
+    //array_u8_alignment (A.split_r slab_region (US.mul (US.mul metadata_max_ex slab_size) n)) (u32_to_sz page_size) /\
+    //zf_u8 (A.asel (A.split_r slab_region (US.mul (US.mul metadata_max_ex slab_size) n)) h1) /\
+    //zf_b (A.asel (A.split_r md_bm_region (US.mul metadata_max_ex n)) h1) /\
+    TLA.length sizes >= US.v offset + US.v n /\
+    synced_sizes offset (asel size_classes h1) sizes (US.v n) /\
     (forall (i:nat{i < US.v n}) . size_class_pred slab_region (Seq.index (asel size_classes h1) i) i)
   )
 
-/// The normalization steps for reduction at compile-time
-unfold
-let normal_steps = [
-      delta_attr [`%reduce_attr];
-      delta_only [`%List.append];
-      iota; zeta; primops]
+#push-options "--fuel 1 --ifuel 1"
+let init_all_size_classes2
+  l offset n slab_region md_bm_region md_region size_classes sizes
+  =
+  f_lemma2 n 0sz;
+  f_lemma2 n 1sz;
+  init_size_classes2 l offset n slab_region md_bm_region md_region size_classes sizes;
+  drop (A.varray (A.split_r slab_region (US.mul (US.mul metadata_max_ex slab_size) n)));
+  drop (A.varray (A.split_r md_bm_region (US.mul metadata_max_ex n)));
+  drop (A.varray (A.split_r md_region (US.mul metadata_max_ex n)))
+#pop-options
 
-unfold
-let normal (#a:Type) (x:a) =
-  Pervasives.norm normal_steps x
+[@"opaque_to_smt"]
+let synced_sizes2
+  (offset: US.t)
+  (size_classes:Seq.seq size_class)
+  (sizes:TLA.t sc_union)
+  (k:nat{
+    k <= Seq.length size_classes /\
+    k + US.v offset <= TLA.length sizes
+  })
+  : prop
+  =
+  synced_sizes offset size_classes sizes k
 
-let init_size_classes l n slab_region md_bm_region md_region size_classes sizes =
-  (normal (init_size_classes_aux l n 0sz 1sz)) slab_region md_bm_region md_region size_classes sizes
+[@"opaque_to_smt"]
+let size_class_preds
+  (size_classes:Seq.seq size_class)
+  (k:nat{k <= Seq.length size_classes})
+  (slab_region: array U8.t{A.length slab_region >= US.v sc_slab_region_size * k})
+  : prop
+  =
+  forall (i:nat{i < k}). (
+    size_class_pred slab_region (Seq.index size_classes i) i
+  )
+
+noextract inline_for_extraction
+val init_all_size_classes_wrapper1 (l:list sc)
+  (offset: US.t)
+  (n: US.t{
+    UInt.size (US.v n) U32.n /\
+    US.fits (US.v n) /\
+    US.fits (US.v metadata_max * US.v (u32_to_sz page_size) * US.v n) /\
+    US.fits (US.v metadata_max * US.v 4sz * US.v n) /\
+    US.fits (US.v metadata_max * US.v n)
+  })
+  (slab_region: array U8.t{
+    A.length slab_region == US.v metadata_max * US.v (u32_to_sz page_size) * US.v n
+  })
+  (md_bm_region: array U64.t{
+    A.length md_bm_region == US.v metadata_max * US.v 4sz * US.v n
+  })
+  (md_region: array AL.cell{
+    A.length md_region == US.v metadata_max * US.v n
+  })
+  (size_classes: array size_class{A.length size_classes == US.v n})
+  (sizes: TLA.t sc_union)
+  //(sizes: array sc{A.length sizes == US.v n})
+  : Steel unit
+  (
+    A.varray slab_region `star`
+    A.varray md_bm_region `star`
+    A.varray md_region `star`
+    A.varray size_classes
+    //`star`
+    //A.varray sizes
+  )
+  (fun r ->
+    A.varray size_classes
+    //`star`
+    //A.varray sizes
+  )
+  (requires fun h0 ->
+    // Invariant needed to link the list against the size classes
+    // allocated in previous iterations
+    List.length l == US.v n /\
+    Cons? l /\
+
+    array_u8_alignment slab_region page_size /\
+    zf_u8 (A.asel slab_region h0) /\
+    zf_u64 (A.asel md_bm_region h0) /\
+    TLA.length sizes >= US.v offset + US.v n /\
+    //synced_sizes (asel size_classes h0) 0 sizes /\
+    //(forall (i:nat{i < US.v n}) . Sc? (Seq.index (asel size_classes h0) i).data.size) /\
+    True
+    //(forall (i:nat{i < 0}) . size_class_pred slab_region (Seq.index (asel size_classes h0) i) i)
+  )
+  (ensures fun _ r h1 ->
+    //array_u8_alignment (A.split_r slab_region (US.mul (US.mul metadata_max (u32_to_sz page_size)) n)) (u32_to_sz page_size) /\
+    //zf_u8 (A.asel (A.split_r slab_region (US.mul (US.mul metadata_max (u32_to_sz page_size)) n)) h1) /\
+    //zf_u64 (A.asel (A.split_r md_bm_region (US.mul (US.mul metadata_max 4sz) n)) h1) /\
+    TLA.length sizes >= US.v offset + US.v n /\
+    synced_sizes2 offset (asel size_classes h1) sizes (US.v n) /\
+    size_class_preds (asel size_classes h1) (US.v n) slab_region
+  )
+
+#push-options "--fuel 1 --ifuel 1"
+let init_all_size_classes_wrapper1
+  l offset n slab_region md_bm_region md_region size_classes sizes
+  =
+  Math.Lemmas.mul_zero_right_is_zero (US.v (US.mul metadata_max (u32_to_sz page_size)));
+  Math.Lemmas.mul_zero_right_is_zero (US.v (US.mul metadata_max 4sz));
+  Math.Lemmas.mul_zero_right_is_zero (US.v metadata_max);
+  A.ptr_shift_zero (A.ptr_of slab_region);
+  A.ptr_shift_zero (A.ptr_of md_bm_region);
+  A.ptr_shift_zero (A.ptr_of md_region);
+
+  change_equal_slprop
+    (A.varray slab_region)
+    (A.varray (A.split_r slab_region (US.mul (US.mul metadata_max (u32_to_sz page_size)) 0sz)));
+  change_equal_slprop
+    (A.varray md_bm_region)
+    (A.varray (A.split_r md_bm_region (US.mul (US.mul metadata_max 4sz) 0sz)));
+  change_equal_slprop
+    (A.varray md_region)
+    (A.varray (A.split_r md_region (US.mul metadata_max 0sz)));
+  init_all_size_classes1 l offset n slab_region md_bm_region md_region size_classes sizes;
+  reveal_opaque (`%synced_sizes2) synced_sizes2;
+  reveal_opaque (`%size_class_preds) size_class_preds
+#pop-options
+
+noextract inline_for_extraction
+val init_all_size_classes_wrapper2 (l:list sc_ex)
+  (offset: US.t)
+  (n: US.t{
+    UInt.size (US.v n) U32.n /\
+    US.fits (US.v n) /\
+    US.fits (US.v metadata_max_ex * US.v slab_size * US.v n) /\
+    US.fits (US.v metadata_max_ex * US.v n)
+  })
+  (slab_region: array U8.t{
+    A.length slab_region == US.v metadata_max_ex * US.v slab_size * US.v n
+  })
+  (md_bm_region: array bool{
+    A.length md_bm_region == US.v metadata_max_ex * US.v n
+  })
+  (md_region: array AL.cell{
+    A.length md_region == US.v metadata_max_ex * US.v n
+  })
+  (size_classes: array size_class{A.length size_classes == US.v n})
+  (sizes: TLA.t sc_union)
+  ///\ TLA.length sizes >= US.v offset /\ TLA.length sizes >= A.length size_classes})
+  //(sizes: array sc{A.length sizes == US.v n})
+  : Steel unit
+  (
+    A.varray slab_region `star`
+    A.varray md_bm_region `star`
+    A.varray md_region `star`
+    A.varray size_classes
+    //`star`
+    //A.varray sizes
+  )
+  (fun r ->
+    A.varray size_classes
+    //`star`
+    //A.varray sizes
+  )
+  (requires fun h0 ->
+    // Invariant needed to link the list against the size classes
+    // allocated in previous iterations
+    List.length l == US.v n /\
+    Cons? l /\
+
+    array_u8_alignment slab_region page_size /\
+    zf_u8 (A.asel slab_region h0) /\
+    zf_b (A.asel md_bm_region h0) /\
+    TLA.length sizes >= US.v offset + US.v n /\
+    True
+    //(forall (i:nat{i < US.v offset}) . size_class_pred slab_region (Seq.index (asel size_classes h0) i) i)
+  )
+  (ensures fun _ r h1 ->
+    //array_u8_alignment (A.split_r slab_region (US.mul (US.mul metadata_max_ex slab_size) n)) (u32_to_sz page_size) /\
+    //zf_u8 (A.asel (A.split_r slab_region (US.mul (US.mul metadata_max_ex slab_size) n)) h1) /\
+    //zf_b (A.asel (A.split_r md_bm_region (US.mul metadata_max_ex n)) h1) /\
+    TLA.length sizes >= US.v offset + US.v n /\
+    synced_sizes2 offset (asel size_classes h1) sizes (US.v n) /\
+    size_class_preds (asel size_classes h1) (US.v n) slab_region
+  )
+
+#push-options "--fuel 1 --ifuel 1"
+let init_all_size_classes_wrapper2
+  l offset n slab_region md_bm_region md_region size_classes sizes
+  =
+  Math.Lemmas.mul_zero_right_is_zero (US.v (US.mul metadata_max_ex slab_size));
+  Math.Lemmas.mul_zero_right_is_zero (US.v metadata_max_ex);
+  A.ptr_shift_zero (A.ptr_of slab_region);
+  A.ptr_shift_zero (A.ptr_of md_bm_region);
+  A.ptr_shift_zero (A.ptr_of md_region);
+
+  change_equal_slprop
+    (A.varray slab_region)
+    (A.varray (A.split_r slab_region (US.mul (US.mul metadata_max_ex slab_size) 0sz)));
+  change_equal_slprop
+    (A.varray md_bm_region)
+    (A.varray (A.split_r md_bm_region (US.mul metadata_max_ex 0sz)));
+  change_equal_slprop
+    (A.varray md_region)
+    (A.varray (A.split_r md_region (US.mul metadata_max_ex 0sz)));
+  init_all_size_classes2 l offset n slab_region md_bm_region md_region size_classes sizes;
+  reveal_opaque (`%synced_sizes2) synced_sizes2;
+  reveal_opaque (`%size_class_preds) size_class_preds
+#pop-options
+
+#restart-solver
+
+val synced_sizes_join_lemma''
+  (offset: US.t)
+  (n: US.t{
+    UInt.size (US.v n) U32.n /\
+    US.fits (US.v offset + US.v n)
+  })
+  (size_classes: Seq.lseq size_class (US.v n))
+  (sizes: TLA.t sc_union)
+  (n1 n2: US.t)
+  (i:US.t{US.v i < US.v n})
+  : Lemma
+  (requires (
+    US.v n1 + US.v n2 == US.v n /\
+    US.v n1 > 0 /\
+    US.v n2 > 0 /\
+    (let scs1, scs2 = Seq.split size_classes (US.v n1) in
+    TLA.length sizes >= US.v n + US.v offset /\
+    synced_sizes2 offset scs1 sizes (US.v n1) /\
+    synced_sizes2 (US.add offset n1) scs2 sizes (US.v n2) /\
+    True
+  )))
+  (ensures (
+    TLA.get sizes (US.add offset i)
+    == (Seq.index size_classes (US.v i)).data.size
+  ))
+
+#restart-solver
+
+#push-options "--fuel 1 --ifuel 1 --z3rlimit 100 --query_stats"
+let synced_sizes_join_lemma''
+  offset n size_classes sizes n1 n2 i
+  =
+  let scs1, scs2 = Seq.split size_classes (US.v n1) in
+  reveal_opaque (`%synced_sizes2) synced_sizes2;
+  if US.v i < US.v n1
+  then (
+    ()
+  ) else (
+    assert (US.v i - US.v n1 < US.v n2);
+    assert (TLA.get sizes (US.add (US.add offset n1) (US.sub i n1))
+    ==
+    (Seq.index scs2 (US.v (US.sub i n1))).data.size);
+    assert (TLA.get sizes (US.add (US.add offset n1) (US.sub i n1))
+    == TLA.get sizes (US.add offset i));
+    Seq.lemma_index_slice size_classes (US.v n1) (US.v n) (US.v i - US.v n1);
+    assert (Seq.index scs2 (US.v (US.sub i n1))
+    ==
+    Seq.index size_classes (US.v i));
+    ()
+  )
+#pop-options
+
+let synced_sizes_join_lemma'
+  (offset: US.t)
+  (n: US.t{
+    UInt.size (US.v n) U32.n /\
+    US.fits (US.v offset + US.v n)
+  })
+  (size_classes: Seq.lseq size_class (US.v n))
+  (sizes: TLA.t sc_union)
+  (n1 n2: US.t)
+  (i:nat{i < US.v n})
+  : Lemma
+  (requires (
+    US.v n1 + US.v n2 == US.v n /\
+    US.v n1 > 0 /\
+    US.v n2 > 0 /\
+    (let scs1, scs2 = Seq.split size_classes (US.v n1) in
+    TLA.length sizes >= US.v n + US.v offset /\
+    synced_sizes2 offset scs1 sizes (US.v n1) /\
+    synced_sizes2 (US.add offset n1) scs2 sizes (US.v n2) /\
+    True
+  )))
+  (ensures
+    US.fits i /\
+    TLA.get sizes (US.add offset (US.uint_to_t i))
+    == (Seq.index size_classes i).data.size
+  )
+  =
+  synced_sizes_join_lemma'' offset n size_classes sizes n1 n2 (US.uint_to_t i)
+
+let synced_sizes_join_lemma
+  (offset: US.t)
+  (n: US.t{
+    UInt.size (US.v n) U32.n /\
+    US.fits (US.v offset + US.v n)
+  })
+  (size_classes: Seq.lseq size_class (US.v n))
+  (sizes: TLA.t sc_union)
+  (n1 n2: US.t)
+  : Lemma
+  (requires
+    US.v n1 + US.v n2 == US.v n /\
+    US.v n1 > 0 /\
+    US.v n2 > 0 /\
+    (let scs1, scs2 = Seq.split size_classes (US.v n1) in
+    TLA.length sizes >= US.v n + US.v offset /\
+    synced_sizes2 offset scs1 sizes (US.v n1) /\
+    synced_sizes2 (US.add offset n1) scs2 sizes (US.v n2) /\
+    True)
+  )
+  (ensures
+    synced_sizes2 offset size_classes sizes (US.v n)
+  )
+  =
+  reveal_opaque (`%synced_sizes2) synced_sizes2;
+  Classical.forall_intro (Classical.move_requires (
+    synced_sizes_join_lemma' offset n size_classes sizes n1 n2
+  ))
+
+val synced_sizes_join
+  (#opened: _)
+  (offset: US.t)
+  (n1: US.t{US.v n1 > 0})
+  (n2: US.t{US.v n2 > 0})
+  (n: US.t{
+    UInt.size (US.v n) U32.n /\
+    US.v n == US.v n1 + US.v n2 /\
+    US.fits (US.v offset + US.v n)
+  })
+  (size_classes: array size_class{A.length size_classes == US.v n})
+  (sizes: TLA.t sc_union)
+  // (s1: Seq.lseq size_class (US.v n1))
+  // (s2: Seq.lseq size_class (US.v n2))
+  : SteelGhost unit opened
+  (
+    A.varray (A.split_l size_classes n1) `star`
+    A.varray (A.split_r size_classes n1)
+  )
+  (fun _ ->
+    A.varray size_classes
+  )
+  (requires fun h0 ->
+    TLA.length sizes >= US.v n + US.v offset /\
+    // s1 `Seq.equal` (asel (A.split_l size_classes n1) h0) /\
+    //s2 `Seq.equal` (asel (A.split_r size_classes n1) h0) /\
+    synced_sizes2 offset (asel (A.split_l size_classes n1) h0) sizes (US.v n1) /\
+    synced_sizes2 (US.add offset n1) (asel (A.split_r size_classes n1) h0) sizes
+(US.v n2)
+  )
+  (ensures fun h0 _ h1 ->
+    TLA.length sizes >= US.v n + US.v offset /\
+    asel size_classes h1 `Seq.equal` Seq.append (asel (A.split_l size_classes n1) h0) (asel (A.split_r size_classes n1) h0) /\
+    synced_sizes2 offset (asel size_classes h1) sizes (US.v n)
+  )
+
+#push-options "--fuel 1 --ifuel 1"
+let synced_sizes_join offset n1 n2 n size_classes sizes
+  =
+  let s1 = gget (A.varray (A.split_l size_classes n1)) in
+  let s2 = gget (A.varray (A.split_r size_classes n1)) in
+  A.ghost_join
+   (A.split_l size_classes n1)
+   (A.split_r size_classes n1)
+   ();
+  change_equal_slprop
+   (A.varray (A.merge
+     (A.split_l size_classes n1)
+     (A.split_r size_classes n1)))
+   (A.varray size_classes);
+  let s = gget (A.varray size_classes) in
+  let s1', s2' = Seq.split s (US.v n1) in
+  Seq.lemma_append_inj s1 s2 s1' s2';
+  synced_sizes_join_lemma offset n s sizes n1 n2
+#pop-options
+
+#restart-solver
+
+#push-options "--fuel 0 --ifuel 0 --z3rlimit 100"
+val slab_region_pred_join_lemma_aux'
+  (n: US.t{
+    US.fits (US.v sc_slab_region_size * US.v n)
+  })
+  (slab_region: array U8.t{A.length slab_region = US.v sc_slab_region_size * US.v n})
+  (size_classes: Seq.lseq size_class (US.v n))
+  (n1 n2: US.t)
+  (_:unit{
+    US.v n1 + US.v n2 == US.v n /\
+    US.v n1 > 0 /\
+    US.fits (US.v sc_slab_region_size * US.v n1) /\
+    US.fits (US.v sc_slab_region_size * US.v n2) /\
+    US.v n2 > 0 /\
+    (let scs1, scs2 = Seq.split size_classes (US.v n1) in
+    (forall (i:nat{i < US.v n1}).
+      size_class_pred (A.split_l slab_region (US.mul sc_slab_region_size n1)) (Seq.index scs1 i) i
+    ) /\
+    A.length (A.split_r slab_region (US.mul sc_slab_region_size n1))
+    == US.v sc_slab_region_size * US.v n2 /\
+    (forall (i:nat{i < US.v n2}).
+      size_class_pred (A.split_r slab_region (US.mul sc_slab_region_size n1)) (Seq.index scs2 i) i
+    ))
+  })
+  (i:nat{i < US.v n})
+  : Lemma
+  (
+    size_class_pred slab_region (Seq.index size_classes i) i
+  )
+#pop-options
+
+#restart-solver
+
+#push-options "--fuel 0 --ifuel 0 --z3rlimit 200"
+let slab_region_pred_join_lemma_aux' n slab_region size_classes n1 n2 _ i
+  =
+  //TODO: low-level proof work
+  admit ();
+  let scs1, scs2 = Seq.split size_classes (US.v n1) in
+  if i < US.v n1
+  then (
+    assert (Seq.index scs1 i == Seq.index size_classes i);
+    assert (A.offset (A.ptr_of (A.split_l slab_region (US.mul sc_slab_region_size n1)))
+    == A.offset (A.ptr_of slab_region))
+  ) else (
+    Seq.lemma_index_slice size_classes (US.v n1) (US.v n) (i - US.v n1);
+    assert (Seq.index scs2 (i - US.v n1)
+    == Seq.index size_classes i);
+    assert (A.offset (A.ptr_of (A.split_r slab_region (US.mul  sc_slab_region_size n1)))
+    == A.offset (A.ptr_of slab_region) + US.v sc_slab_region_size * US.v n1);
+    assert (A.offset (A.ptr_of (A.split_r slab_region (US.mul sc_slab_region_size n1))) + US.v sc_slab_region_size * (i - US.v n1)
+    ==
+    A.offset (A.ptr_of slab_region) + US.v sc_slab_region_size * i)
+  )
+#pop-options
+
+#push-options "--fuel 0 --ifuel 0 --z3rlimit 300"
+val slab_region_pred_join_lemma'
+  (n: US.t{
+    US.fits (US.v sc_slab_region_size * US.v n)
+  })
+  (slab_region: array U8.t{A.length slab_region == US.v sc_slab_region_size * US.v n})
+  (size_classes: Seq.lseq size_class (US.v n))
+  (n1 n2: US.t)
+  : Lemma
+  (requires
+    US.v n1 + US.v n2 == US.v n /\
+    US.v n1 > 0 /\
+    US.v n2 > 0 /\
+    US.fits (US.v sc_slab_region_size * US.v n1) /\
+    US.fits (US.v sc_slab_region_size * US.v n2) /\
+    (let scs1, scs2 = Seq.split size_classes (US.v n1) in
+    (forall (i:nat{i < US.v n1}).
+      size_class_pred (A.split_l slab_region (US.mul sc_slab_region_size n1)) (Seq.index scs1 i) i
+    ) /\
+    (forall (i:nat{i < US.v n2}).
+      size_class_pred (A.split_r slab_region (US.mul sc_slab_region_size n1)) (Seq.index scs2 i) i
+    ))
+  )
+  (ensures
+    forall (i:nat{i < US.v n}).
+      size_class_pred slab_region (Seq.index size_classes i) i
+  )
+#pop-options
+
+#push-options "--fuel 1 --ifuel 1 --z3rlimit 50"
+let slab_region_pred_join_lemma' n slab_region size_classes n1 n2
+  =
+  //TODO: low-level proof work
+  admit ();
+  Classical.forall_intro (Classical.move_requires (
+    slab_region_pred_join_lemma_aux' n slab_region size_classes n1 n2 ()
+  ))
+#pop-options
+
+#push-options "--fuel 0 --ifuel 0 --z3rlimit 300"
+val slab_region_pred_join_lemma
+  (n1 n2: US.t)
+  (n: US.t{
+    US.fits (US.v sc_slab_region_size * US.v n)
+  })
+  (slab_region: array U8.t{A.length slab_region == US.v sc_slab_region_size * US.v n})
+  (size_classes: Seq.lseq size_class (US.v n))
+  : Lemma
+  (requires
+    US.v n1 + US.v n2 == US.v n /\
+    US.v n1 > 0 /\
+    US.v n2 > 0 /\
+    US.fits (US.v sc_slab_region_size * US.v n1) /\
+    US.fits (US.v sc_slab_region_size * US.v n2) /\
+    (let scs = Seq.split size_classes (US.v n1) in
+      size_class_preds (fst scs) (US.v n1) (A.split_l slab_region (US.mul sc_slab_region_size n1)) /\
+      size_class_preds (snd scs) (US.v n2) (A.split_r slab_region (US.mul sc_slab_region_size n1))
+    )
+  )
+  (ensures
+    size_class_preds size_classes (US.v n) slab_region
+  )
+#pop-options
+
+let slab_region_pred_join_lemma n1 n2 n slab_region size_classes
+  =
+  reveal_opaque (`%size_class_preds) size_class_preds;
+  slab_region_pred_join_lemma' n slab_region size_classes n1 n2
+
+#restart-solver
+
+(*
+so far, so good, with the exception of:
+- sc? and sc_ex? pattern: use a opaque predicate
+*)
+
+#push-options "--fuel 0 --ifuel 0 --z3rlimit 300"
+val init_all_size_classes'
+  (#opened:_)
+  (offset: US.t)
+  (n1: US.t{US.v n1 > 0})
+  (n2: US.t{US.v n2 > 0})
+  (n: US.t{
+    US.v n == US.v n1 + US.v n2 /\
+    UInt.size (US.v n) U32.n /\
+    US.fits (US.v sc_slab_region_size * US.v n) /\
+    //US.fits (US.v sc_slab_region_size * US.v n1) /\
+    //US.fits (US.v sc_slab_region_size * US.v n2) /\
+    US.fits (US.v n + US.v offset)
+  })
+  (slab_region: array U8.t{
+    A.length slab_region == US.v sc_slab_region_size * US.v n /\
+    A.length slab_region >= US.v sc_slab_region_size * US.v n1 /\
+    A.length slab_region >= US.v sc_slab_region_size * US.v n2 /\
+    True
+  })
+  (size_classes: array size_class{A.length size_classes == US.v n})
+  (sizes: TLA.t sc_union)
+  : SteelGhost unit opened
+  (
+    A.varray (A.split_l size_classes n1) `star`
+    A.varray (A.split_r size_classes n1)
+  )
+  (fun _ ->
+    A.varray size_classes
+  )
+  (requires fun h0 ->
+    A.length (A.split_l slab_region (US.mul sc_slab_region_size n1)) == US.v sc_slab_region_size * US.v n1 /\
+    A.length (A.split_r slab_region (US.mul sc_slab_region_size n1)) == US.v sc_slab_region_size * US.v n2 /\
+    TLA.length sizes >= US.v n + US.v offset /\
+    synced_sizes2 offset
+      (asel (A.split_l size_classes n1) h0) sizes (US.v n1) /\
+    synced_sizes2 (US.add offset n1)
+      (asel (A.split_r size_classes n1) h0) sizes (US.v n2) /\
+    size_class_preds (asel (A.split_l size_classes n1) h0) (US.v n1) (A.split_l slab_region (US.mul sc_slab_region_size n1)) /\
+    size_class_preds (asel (A.split_r size_classes n1) h0) (US.v n2) (A.split_r slab_region (US.mul sc_slab_region_size n1)) /\
+    True
+    //(forall (i:nat{i < US.v n1}).
+    //  size_class_pred (A.split_l slab_region (US.mul n1 sc_slab_region_size)) (Seq.index (asel (A.split_l size_classes n1) h0) i) i
+    //)
+    ///\
+    //(forall (i:nat{i < US.v n2}).
+    //  size_class_pred (A.split_r slab_region (US.mul n1 sc_slab_region_size)) (Seq.index (asel (A.split_r size_classes n1) h0) i) i
+    //)
+  )
+  (ensures fun _ _ h1 ->
+    TLA.length sizes >= US.v n + US.v offset /\
+    synced_sizes2 offset (asel size_classes h1) sizes (US.v n) /\
+    size_class_preds (asel size_classes h1) (US.v n) slab_region
+  )
+#pop-options
+
+#restart-solver
+
+//[@@ handle_smt_goals]
+//let tac () : FStar.Tactics.Tac unit = FStar.Tactics.norm [zeta_full; delta_only [`%focus_rmem; `%focus_rmem'; `%unrestricted_focus_rmem]]
+
+#push-options "--fuel 1 --ifuel 1 --z3rlimit 300 --query_stats"
+let init_all_size_classes'
+  offset
+  n1 n2 n
+  slab_region
+  size_classes
+  sizes
+  =
+  let size_classes1_s0 = gget (A.varray (A.split_l size_classes n1)) in
+  let size_classes2_s0 = gget (A.varray (A.split_r size_classes n1)) in
+  synced_sizes_join offset n1 n2 n size_classes sizes;
+  let size_classes_s1 = gget (A.varray size_classes) in
+  assert (G.reveal size_classes_s1 == Seq.append size_classes1_s0 size_classes2_s0);
+  Seq.lemma_split size_classes_s1 (US.v n1);
+  let size_classes1_s1, size_classes2_s1 = Seq.split size_classes_s1 (US.v n1) in
+  Seq.lemma_append_inj
+    size_classes1_s0 size_classes2_s0
+    size_classes1_s1 size_classes2_s1;
+  assert (G.reveal size_classes1_s0 == size_classes1_s1);
+  assert (G.reveal size_classes2_s0 == size_classes2_s1);
+  slab_region_pred_join_lemma n1 n2 n slab_region size_classes_s1
+#pop-options
+
+// OK
+
+noextract inline_for_extraction
+val init_all_size_classes
+  (l1:list sc)
+  (l2:list sc_ex)
+  (offset: US.t)
+  (n: US.t{
+    US.v n == List.length l1 + List.length l2 /\
+    UInt.size (US.v n) U32.n /\
+    US.fits (US.v n + US.v offset) /\
+    US.fits (US.v metadata_max * US.v (u32_to_sz page_size) * US.v n) /\
+    US.fits (US.v metadata_max * US.v 4sz * US.v n) /\
+    US.fits (US.v metadata_max * US.v n)
+  })
+  (n1: US.t{US.v n1 == List.length l1 /\ US.v n1 > 0})
+  (n2: US.t{US.v n2 == List.length l2 /\ US.v n2 > 0})
+  (slab_region: array U8.t{
+    A.length slab_region == US.v metadata_max * US.v (u32_to_sz page_size) * US.v n
+  })
+  (md_bm_region: array U64.t{
+    A.length md_bm_region == US.v metadata_max * US.v 4sz * US.v n1
+  })
+  (md_bm_region_b: array bool{
+    A.length md_bm_region_b == US.v metadata_max_ex * US.v n2
+  })
+  (md_region: array AL.cell{
+    A.length md_region == US.v metadata_max * US.v n1 + US.v metadata_max_ex * US.v n2
+  })
+  (size_classes: array size_class{A.length size_classes == US.v n})
+  (sizes: TLA.t sc_union)
+  : Steel unit
+  (
+    A.varray (A.split_l slab_region (US.mul (US.mul metadata_max (u32_to_sz page_size)) n1)) `star`
+    A.varray (A.split_r slab_region (US.mul (US.mul metadata_max (u32_to_sz page_size)) n1)) `star`
+    A.varray md_bm_region `star`
+    A.varray md_bm_region_b `star`
+    A.varray (A.split_l md_region (US.mul metadata_max n1)) `star`
+    A.varray (A.split_r md_region (US.mul metadata_max n1)) `star`
+    A.varray (A.split_l size_classes n1) `star`
+    A.varray (A.split_r size_classes n1)
+  )
+  (fun _ ->
+    A.varray size_classes
+  )
+  (requires fun h0 ->
+    Cons? l1 /\
+    Cons? l2 /\
+    US.v n1 > 0 /\
+    US.v n2 > 0 /\
+    array_u8_alignment (A.split_l slab_region (US.mul (US.mul metadata_max (u32_to_sz page_size)) n1)) page_size /\
+    array_u8_alignment (A.split_r slab_region (US.mul (US.mul metadata_max (u32_to_sz page_size)) n1)) page_size /\
+    zf_u8 (A.asel (A.split_l slab_region (US.mul (US.mul metadata_max (u32_to_sz page_size)) n1)) h0) /\
+    zf_u8 (A.asel (A.split_r slab_region (US.mul (US.mul metadata_max (u32_to_sz page_size)) n1)) h0) /\
+    zf_u64 (A.asel md_bm_region h0) /\
+    zf_b (A.asel md_bm_region_b h0) /\
+    TLA.length sizes >= US.v n + US.v offset /\
+    //(forall (i:nat{i < US.v n1}) . Sc? (Seq.index (asel (A.split_l size_classes n1) h0) i).data.size) /\
+    //(forall (i:nat{i < US.v n2}) . Sc_ex? (Seq.index (asel (A.split_r size_classes n1) h0) i).data.size) /\
+    True
+  )
+  (ensures fun _ _ h1 ->
+    TLA.length sizes >= US.v n + US.v offset /\
+    synced_sizes2 offset (asel size_classes h1) sizes (US.v n) /\
+    size_class_preds (asel size_classes h1) (US.v n) slab_region
+    //(forall (i:nat{i < US.v n}) . size_class_pred slab_region (Seq.index (asel size_classes h1) i) i)
+  )
+
+#restart-solver
+
+#restart-solver
+
+#push-options "--fuel 0 --ifuel 0 --z3rlimit 500"
+let init_all_size_classes
+  l1 l2
+  offset
+  n n1 n2
+  slab_region
+  md_bm_region
+  md_bm_region_b
+  md_region
+  size_classes
+  sizes
+  =
+  init_all_size_classes_wrapper1 l1 offset n1
+    (A.split_l slab_region (US.mul (US.mul metadata_max (u32_to_sz page_size)) n1))
+    md_bm_region
+    (A.split_l md_region (US.mul metadata_max n1))
+    (A.split_l size_classes n1)
+    sizes;
+  //TODO: dedicated lemma
+  assume (A.length (A.split_r slab_region (US.mul (US.mul metadata_max (u32_to_sz page_size)) n1))
+  ==
+  US.v metadata_max_ex * US.v slab_size * US.v n2);
+  //TODO: dedicated lemma
+  assume (A.length (A.split_r md_region (US.mul metadata_max n1))
+  ==
+  US.v metadata_max_ex * US.v n2);
+  //TODO: dedicated lemma
+  assume (A.length (A.split_r size_classes n1) == US.v n2);
+  init_all_size_classes_wrapper2 l2 (US.add offset n1) n2
+    (A.split_r slab_region (US.mul (US.mul metadata_max (u32_to_sz page_size)) n1))
+    md_bm_region_b
+    (A.split_r md_region (US.mul metadata_max n1))
+    (A.split_r size_classes n1)
+    sizes;
+  init_all_size_classes'
+    offset
+    n1 n2 n
+    slab_region
+    size_classes
+    sizes
+#pop-options
+
+noextract inline_for_extraction
+val init_all_size_classes_wrapper
+  (l1:list sc)
+  (l2:list sc_ex)
+  (offset: US.t)
+  (n: US.t{
+    US.v n == List.length l1 + List.length l2 /\
+    UInt.size (US.v n) U32.n /\
+    US.fits (US.v n + US.v offset) /\
+    US.fits (US.v metadata_max * US.v (u32_to_sz page_size) * US.v n) /\
+    US.fits (US.v metadata_max * US.v 4sz * US.v n) /\
+    US.fits (US.v metadata_max * US.v n)
+  })
+  (n1: US.t{US.v n1 == List.length l1})
+  (n2: US.t{US.v n2 == List.length l2})
+  (slab_region: array U8.t{
+    A.length slab_region == US.v metadata_max * US.v (u32_to_sz page_size) * US.v n
+  })
+  (md_bm_region: array U64.t{
+    A.length md_bm_region == US.v metadata_max * US.v 4sz * US.v n1
+  })
+  (md_bm_region_b: array bool{
+    A.length md_bm_region_b == US.v metadata_max_ex * US.v n2
+  })
+  (md_region: array AL.cell{
+    A.length md_region == US.v metadata_max * US.v n1 + US.v metadata_max_ex * US.v n2
+  })
+  (size_classes: array size_class{A.length size_classes == US.v n})
+  (sizes: TLA.t sc_union)
+  : Steel unit
+  (
+    A.varray slab_region `star`
+    A.varray md_bm_region `star`
+    A.varray md_bm_region_b `star`
+    A.varray md_region `star`
+    A.varray size_classes
+  )
+  (fun _ ->
+    A.varray size_classes
+  )
+  (requires fun h0 ->
+    Cons? l1 /\
+    Cons? l2 /\
+    US.v n1 > 0 /\
+    US.v n2 > 0 /\
+    array_u8_alignment slab_region page_size /\
+    zf_u8 (A.asel slab_region h0) /\
+    zf_u64 (A.asel md_bm_region h0) /\
+    zf_b (A.asel md_bm_region_b h0) /\
+    TLA.length sizes >= US.v n + US.v offset /\
+    //(forall (i:nat{i < US.v n1}) . Sc? (Seq.index (asel size_classes h0) i).data.size) /\
+    //(forall (i:nat{i >= US.v n1 /\ i < US.v n}) . Sc_ex? (Seq.index (asel size_classes h0) i).data.size) /\
+    True
+  )
+  (ensures fun _ _ h1 ->
+    TLA.length sizes >= US.v n + US.v offset /\
+    synced_sizes2 offset (asel size_classes h1) sizes (US.v n) /\
+    size_class_preds (asel size_classes h1) (US.v n) slab_region
+  )
+
+
+#restart-solver
+
+#push-options "--fuel 0 --ifuel 0 --z3rlimit 200"
+let init_all_size_classes_wrapper
+  l1 l2
+  offset
+  n n1 n2
+  slab_region
+  md_bm_region
+  md_bm_region_b
+  md_region
+  size_classes
+  sizes
+  =
+  let slab_region_s0 = gget (A.varray slab_region) in
+  f_lemma n n1;
+  zf_u8_split
+    slab_region_s0
+    (US.v (US.mul (US.mul metadata_max (u32_to_sz page_size)) n1));
+  A.ghost_split slab_region
+    (US.mul (US.mul metadata_max (u32_to_sz page_size)) n1);
+  A.ghost_split md_region
+    (US.mul metadata_max n1);
+  A.ghost_split size_classes n1;
+  //TODO: dedicated lemma
+  assume (array_u8_alignment (A.split_l slab_region (US.mul (US.mul metadata_max (u32_to_sz page_size)) n1)) page_size);
+  //TODO: dedicated lemma
+  assume (array_u8_alignment (A.split_r slab_region (US.mul (US.mul metadata_max (u32_to_sz page_size)) n1)) page_size);
+  let size_classes1_s0 = gget (A.varray (A.split_l size_classes n1)) in
+  let size_classes2_s0 = gget (A.varray (A.split_r size_classes n1)) in
+  init_all_size_classes
+    l1 l2
+    offset
+    n n1 n2
+    slab_region
+    md_bm_region
+    md_bm_region_b
+    md_region
+    size_classes
+    sizes
+#pop-options
+
+// so far, initialization of one arena
+// now, initialization of several arenas
+
+#restart-solver
+
+
+(*
+so far, so good, with the exception of:
+- sc? and sc_ex? pattern: use a opaque predicate
+*)
+
+/// A logical predicate indicating that a list of sizes corresponds
+/// to the sizes of a list of size_classes
+[@"opaque_to_smt"]
+let hidden_pred
+  (l1: list sc)
+  (l2: list sc_ex)
+  (n n1 n2 s1 s2 s3: US.t)
+  : prop
+  =
+  US.fits (US.v metadata_max * US.v (u32_to_sz page_size) * US.v n) /\
+  US.fits (US.v metadata_max * US.v 4sz * US.v n) /\
+  US.fits (US.v metadata_max * US.v n) /\
+  US.v n1 == List.length l1 /\ US.v n1 > 0 /\
+  US.v n2 == List.length l2 /\ US.v n2 > 0 /\
+  US.v n == US.v n1 + US.v n2 /\
+  Cons? l1 /\
+  Cons? l2 /\
+  US.v n == List.length l1 + List.length l2 /\
+  // arena_slab_region_size
+  //US.v s1 == US.v sc_slab_region_size * US.v n /\
+  // arena md_bm_region size
+  US.v s1 == US.v metadata_max * US.v 4sz * US.v n1 /\
+  // arena md_bm_region_b size
+  US.v s2 == US.v metadata_max_ex * US.v n2 /\
+  // arena md_region size
+  US.v s3 == US.v metadata_max * US.v n1 + US.v metadata_max_ex * US.v n2
+
+noextract inline_for_extraction
+val init_one_arena'
+  (offset: US.t)
+  (l1:list sc)
+  (l2:list sc_ex)
+  (n1 n2: US.t)
+  (n: US.t{
+    US.v n > 0 /\
+    UInt.size (US.v n) U32.n /\
+    US.fits (US.v n + US.v offset)
+  })
+  (arena_slab_region_size
+   arena_md_region_size
+   arena_md_bm_region_size
+   arena_md_bm_region_b_size: (v:US.t{US.v v > 0}))
+  (slab_region: array U8.t{
+    A.length slab_region == US.v arena_slab_region_size
+  })
+  (md_bm_region: array U64.t{
+    A.length md_bm_region == US.v arena_md_bm_region_size
+  })
+  (md_bm_region_b: array bool{
+    A.length md_bm_region_b == US.v arena_md_bm_region_b_size
+  })
+  (md_region: array AL.cell{
+    A.length md_region == US.v arena_md_region_size
+  })
+  (size_classes: array size_class{A.length size_classes == US.v n})
+  (sizes: TLA.t sc_union)
+  : Steel unit
+  (
+    A.varray slab_region `star`
+    A.varray md_bm_region `star`
+    A.varray md_bm_region_b `star`
+    A.varray md_region `star`
+    A.varray size_classes
+  )
+  (fun _ ->
+    A.varray size_classes
+  )
+  (requires fun h0 ->
+    //(forall (i:nat{i < US.v n1}) . Sc? (Seq.index (asel size_classes h0) i).data.size) /\
+    //(forall (i:nat{i >= US.v n1 /\ i < US.v n}) . Sc_ex? (Seq.index (asel size_classes h0) i).data.size) /\
+    array_u8_alignment slab_region page_size /\
+    zf_u8 (A.asel slab_region h0) /\
+    zf_u64 (A.asel md_bm_region h0) /\
+    zf_b (A.asel md_bm_region_b h0) /\
+    TLA.length sizes >= US.v n + US.v offset /\
+    US.v arena_slab_region_size == US.v sc_slab_region_size * US.v n /\
+    hidden_pred l1 l2 n n1 n2
+      arena_md_bm_region_size
+      arena_md_bm_region_b_size
+      arena_md_region_size
+  )
+  (ensures fun _ _ h1 ->
+    TLA.length sizes >= US.v n + US.v offset /\
+    A.length slab_region >= US.v sc_slab_region_size * US.v n /\
+    synced_sizes2 offset (asel size_classes h1) sizes (US.v n) /\
+    size_class_preds (asel size_classes h1) (US.v n) slab_region
+  )
+
+// OK
+
+#push-options "--fuel 0 --ifuel 0 --z3rlimit 400"
+let init_one_arena'
+  offset
+  l1 l2 n1 n2 n
+  (arena_slab_region_size
+   arena_md_region_size
+   arena_md_bm_region_size
+   arena_md_bm_region_b_size: (v:US.t{US.v v > 0}))
+  slab_region
+  md_bm_region
+  md_bm_region_b
+  md_region
+  size_classes
+  sizes
+  =
+  reveal_opaque (`%hidden_pred) hidden_pred;
+  init_all_size_classes_wrapper
+    l1 l2
+    offset
+    n n1 n2
+    slab_region
+    md_bm_region
+    md_bm_region_b
+    md_region
+    size_classes
+    sizes
+#pop-options
+
+#restart-solver
+
+//[@"opaque_to_smt"]
+//let sc_list_layout1
+//  (n1 n2: (v:US.t{US.v v > 0}))
+//  (n: US.t{US.v n == US.v n1 + US.v n2})
+//  (sizes: TLA.t sc_union{TLA.length sizes == US.v n})
+//  : prop
+//  =
+//  (forall (i:US.t{US.v i < US.v n1}).
+//    Sc? (TLA.get sizes i)) /\
+//  (forall (i:US.t{US.v i >= US.v n1 /\ US.v i < US.v n}).
+//    Sc_ex? (TLA.get sizes i))
+//
+//#push-options "--fuel 0 --ifuel 0 --z3rlimit 300"
+//[@"opaque_to_smt"]
+//let sc_list_layout2
+//  (nb_arenas: US.t{US.v nb_arenas > 0})
+//  (n1 n2: (v:US.t{US.v v > 0}))
+//  (n: US.t{US.v n == US.v n1 + US.v n2})
+//  (sizes: TLA.t sc_union{
+//    US.fits (US.v nb_arenas * US.v n) /\
+//    TLA.length sizes == US.v nb_arenas * US.v n
+//  })
+//  : prop
+//  =
+//  (forall (k:US.t{US.v k < US.v nb_arenas}).
+//    US.fits (US.v nb_arenas * US.v k) /\
+//    (forall (i: US.t{US.v i < US.v n1}).
+//      US.fits (US.v nb_arenas * US.v k + US.v i) /\
+//      US.v nb_arenas * US.v k + US.v i < TLA.length sizes /\
+//      Sc? (TLA.get sizes (US.add (US.mul nb_arenas k) i))
+//    ) /\
+//    (forall (i: US.t{US.v i >= US.v n1 /\ US.v i < US.v n}).
+//      US.fits (US.v nb_arenas * US.v k + US.v i) /\
+//      US.v nb_arenas * US.v k + US.v i < TLA.length sizes /\
+//      Sc_ex? (TLA.get sizes (US.add (US.mul nb_arenas k) i))
+//    )
+//  )
+//#pop-options
+//
+//let sc_list_layout_lemma
+//  (nb_arenas: US.t{US.v nb_arenas > 1})
+//  (n1 n2: (v:US.t{US.v v > 0}))
+//  (n: US.t{US.v n == US.v n1 + US.v n2})
+//  (sizes: TLA.t sc_union{
+//    US.fits (US.v nb_arenas * US.v n) /\
+//    TLA.length sizes == US.v nb_arenas * US.v n
+//  })
+//  : Lemma
+//  (requires sc_list_layout2 nb_arenas n1 n2 n sizes)
+//  (ensures (
+//    let sizes1, sizes2 = TLAO.split sizes (US.v n) in
+//    sc_list_layout1 n1 n2 n sizes1))
+//  = admit ()
+
+#push-options "--fuel 0 --ifuel 0 --z3rlimit 300"
+noextract inline_for_extraction
+val init_one_arena
+  (offset: US.t)
+  (l1:list sc)
+  (l2:list sc_ex)
+  (n1 n2: US.t)
+  (n: US.t{
+    US.v n > 0 /\
+    UInt.size (US.v n) U32.n /\
+    US.fits (US.v n + US.v offset)
+  })
+  (nb_arenas: US.t{US.v nb_arenas > 0})
+  (arena_slab_region_size
+   arena_md_region_size
+   arena_md_bm_region_size
+   arena_md_bm_region_b_size: (v:US.t{US.v v > 0}))
+  (slab_region: array U8.t{
+    A.length slab_region >= US.v arena_slab_region_size
+  })
+  (md_bm_region: array U64.t{
+    A.length md_bm_region >= US.v arena_md_bm_region_size
+  })
+  (md_bm_region_b: array bool{
+    A.length md_bm_region_b >= US.v arena_md_bm_region_b_size
+  })
+  (md_region: array AL.cell{
+    A.length md_region >= US.v arena_md_region_size
+  })
+  (size_classes: array size_class{
+    A.length size_classes >= US.v n
+  })
+  (sizes: TLA.t sc_union)//{TLA.length sizes == US.v n * US.v nb_arenas})
+  : Steel unit
+  (
+    A.varray slab_region `star`
+    A.varray md_bm_region `star`
+    A.varray md_bm_region_b `star`
+    A.varray md_region `star`
+    A.varray size_classes
+  )
+  (fun _ ->
+    A.varray (A.split_r slab_region arena_slab_region_size) `star`
+    A.varray (A.split_r md_bm_region arena_md_bm_region_size) `star`
+    A.varray (A.split_r md_bm_region_b arena_md_bm_region_b_size) `star`
+    A.varray (A.split_r md_region arena_md_region_size) `star`
+    //A.varray (A.split_l size_classes n) `star`
+    //A.varray (A.split_r size_classes n)
+    A.varray size_classes
+  )
+  (requires fun h0 ->
+    array_u8_alignment slab_region page_size /\
+    zf_u8 (A.asel slab_region h0) /\
+    zf_u64 (A.asel md_bm_region h0) /\
+    zf_b (A.asel md_bm_region_b h0) /\
+    US.v arena_slab_region_size == US.v sc_slab_region_size * US.v n /\
+    hidden_pred l1 l2 n n1 n2
+      arena_md_bm_region_size
+      arena_md_bm_region_b_size
+      arena_md_region_size /\
+    //US.v n1 + US.v n2 == US.v n /\
+    TLA.length sizes >= US.v n + US.v offset /\
+    A.length size_classes >= US.v n /\
+    //sc_list_layout1 n1 n2 n
+    //(forall (i:nat{i < US.v n1}) . Sc? (Seq.index (asel size_classes h0) i).data.size) /\
+    //(forall (i:nat{i >= US.v n1 /\ i < US.v n}) . Sc_ex? (Seq.index (asel size_classes h0) i).data.size) /\
+    True
+    //(forall (k:nat{k < US.v nb_arenas}).
+    //  (forall (i:nat{i < US.v n1}) .
+    //    Sc? (Seq.index (asel size_classes h0) (k * US.v nb_arenas + i)).data.size) /\
+    //  (forall (i:nat{i >= US.v n1 /\ i < US.v n}) .
+    //    Sc_ex? (Seq.index (asel size_classes h0) (k * US.v nb_arenas + i)).data.size)
+    //)
+  )
+  (ensures fun _ _ h1 ->
+    array_u8_alignment (A.split_r slab_region arena_slab_region_size) page_size /\
+    zf_u8 (A.asel (A.split_r slab_region arena_slab_region_size) h1) /\
+    zf_u64 (A.asel (A.split_r md_bm_region arena_md_bm_region_size) h1) /\
+    zf_b (A.asel (A.split_r md_bm_region_b arena_md_bm_region_b_size) h1) /\
+    TLA.length sizes >= US.v n + US.v offset /\
+    A.length size_classes >= US.v n /\
+    A.length slab_region >= US.v sc_slab_region_size * US.v n /\
+    synced_sizes2 offset (asel size_classes h1) sizes (US.v n) /\
+    size_class_preds (asel size_classes h1) (US.v n) slab_region
+  )
+#pop-options
+
+#restart-solver
+
+#restart-solver
+
+let synced_sizes2_extend_lemma
+  (offset: US.t)
+  (size_classes1 size_classes2:Seq.seq size_class)
+  (sizes:TLA.t sc_union)
+  (k:nat{
+    k <= Seq.length size_classes1 /\
+    k <= Seq.length size_classes2 /\
+    k + US.v offset <= TLA.length sizes
+  })
+  : Lemma
+  (requires
+    Seq.slice size_classes1 0 k
+    ==
+    Seq.slice size_classes2 0 k /\
+    synced_sizes2 offset size_classes1 sizes k
+  )
+  (ensures
+    synced_sizes2 offset size_classes2 sizes k
+  )
+  =
+  Classical.forall_intro (SeqUtils.lemma_index_slice size_classes1 0 k);
+  Classical.forall_intro (SeqUtils.lemma_index_slice size_classes2 0 k);
+  //TODO: low-level proof work
+  assume (forall (i:nat{i < k}).
+    Seq.index size_classes1 i
+    ==
+    Seq.index size_classes2 i
+  );
+  reveal_opaque (`%synced_sizes2) synced_sizes2
+
+let size_class_preds_extend_lemma
+  (size_classes1 size_classes2:Seq.seq size_class)
+  (k:nat{
+    k <= Seq.length size_classes1 /\
+    k <= Seq.length size_classes2
+  })
+  (slab_region1 slab_region2: (v:array U8.t{A.length v >= US.v sc_slab_region_size * k}))
+  : Lemma
+  (requires
+    Seq.slice size_classes1 0 k
+    ==
+    Seq.slice size_classes2 0 k /\
+    A.offset (A.ptr_of slab_region1)
+    ==
+    A.offset (A.ptr_of slab_region2) /\
+    same_base_array slab_region1 slab_region2 /\
+    size_class_preds size_classes1 k slab_region1
+  )
+  (ensures
+    size_class_preds size_classes2 k slab_region2
+  )
+  =
+  //TODO: low-level proof work
+  assume (forall (i:nat{i < k}).
+    Seq.index size_classes1 i
+    ==
+    Seq.index size_classes2 i
+  );
+  reveal_opaque (`%size_class_preds) size_class_preds
+
+#push-options "--fuel 0 --ifuel 0 --z3rlimit 300"
+let init_one_arena
+  offset
+  l1 l2 n1 n2 n
+  nb_arenas
+  (arena_slab_region_size
+   arena_md_region_size
+   arena_md_bm_region_size
+   arena_md_bm_region_b_size: (v:US.t{US.v v > 0}))
+  slab_region
+  md_bm_region
+  md_bm_region_b
+  md_region
+  size_classes
+  sizes
+  =
+  let slab_region_s = gget (A.varray slab_region) in
+  let md_bm_region_s = gget (A.varray md_bm_region) in
+  let md_bm_region_b_s = gget (A.varray md_bm_region_b) in
+  zf_u8_split slab_region_s (US.v arena_slab_region_size);
+  zf_u64_split md_bm_region_s (US.v arena_md_bm_region_size);
+  zf_b_split md_bm_region_b_s (US.v arena_md_bm_region_b_size);
+  A.ghost_split slab_region arena_slab_region_size;
+  A.ghost_split md_bm_region arena_md_bm_region_size;
+  A.ghost_split md_bm_region_b arena_md_bm_region_b_size;
+  A.ghost_split md_region arena_md_region_size;
+  A.ghost_split size_classes n;
+  //TODO: dedicated lemma
+  assume (array_u8_alignment (A.split_l slab_region arena_slab_region_size) page_size);
+  //TODO: dedicated lemma
+  assume (array_u8_alignment (A.split_r slab_region arena_slab_region_size) page_size);
+  init_one_arena'
+    offset
+    l1 l2 n1 n2 n
+    arena_slab_region_size
+    arena_md_region_size
+    arena_md_bm_region_size
+    arena_md_bm_region_b_size
+    (A.split_l slab_region arena_slab_region_size)
+    (A.split_l md_bm_region arena_md_bm_region_size)
+    (A.split_l md_bm_region_b arena_md_bm_region_b_size)
+    (A.split_l md_region arena_md_region_size)
+    (A.split_l size_classes n)
+    sizes;
+  let s1 = gget (A.varray (A.split_l size_classes n)) in
+  let s2 = gget (A.varray (A.split_r size_classes n)) in
+  A.ghost_join
+   (A.split_l size_classes n)
+   (A.split_r size_classes n)
+   ();
+  change_equal_slprop
+   (A.varray (A.merge
+     (A.split_l size_classes n)
+     (A.split_r size_classes n)))
+   (A.varray size_classes);
+  let s = gget (A.varray size_classes) in
+  let s1', s2' = Seq.split s (US.v n) in
+  Seq.lemma_append_inj s1 s2 s1' s2';
+  Seq.lemma_split s (US.v n);
+  assert (Seq.slice s 0 (US.v n) == Seq.slice s1 0 (US.v n));
+  synced_sizes2_extend_lemma offset
+    s1 s
+    sizes
+    (US.v n);
+  size_class_preds_extend_lemma
+    s1 s
+    (US.v n)
+    (A.split_l slab_region arena_slab_region_size)
+    slab_region;
+  ()
+
+[@"opaque_to_smt"]
+let hidden_pred2
+  (n s1: US.t)
+  : prop
+  =
+  US.v n > 0 /\
+  US.v s1 > 0 /\
+  US.v s1 == US.v sc_slab_region_size * US.v n
+
+// predicate:
+// sizes of k arenas after the offset-nth one
+// are properly synced
+[@"opaque_to_smt"]
+let synced_sizes_arena
+  (n: US.t)
+  (offset: US.t)
+  (size_classes:Seq.seq size_class)
+  (sizes:TLA.t sc_union)
+  (k:nat{
+    US.v n * k <= Seq.length size_classes /\
+    US.v n * (k + US.v offset) <= TLA.length sizes /\
+    US.fits (US.v n * (US.v offset + k)) /\
+    //US.fits (US.v n * US.v offset)
+    True
+  })
+  : prop
+  =
+  assert (US.v n * k + US.v (US.mul n offset) <= TLA.length sizes);
+  synced_sizes2 (US.mul n offset) size_classes sizes (US.v n * k)
+
+// predicate:
+//
+
+[@"opaque_to_smt"]
+let size_class_preds_arena
+  (n: US.t)
+  (arena_slab_region_size: US.t)
+  (size_classes:Seq.seq size_class)
+  (k:nat{
+    US.v n * k <= Seq.length size_classes /\
+    hidden_pred2 n arena_slab_region_size
+  })
+  (slab_region: array U8.t{A.length slab_region >= US.v arena_slab_region_size * k})
+  : prop
+  =
+  reveal_opaque (`%hidden_pred2) hidden_pred2;
+  assert (US.v sc_slab_region_size * (US.v n * k)
+  == (US.v sc_slab_region_size * US.v n) * k);
+  assert (US.v sc_slab_region_size * (US.v n * k)
+  == US.v arena_slab_region_size * k);
+  size_class_preds size_classes (US.v n * k) slab_region
+
+noextract inline_for_extraction
+val init_one_arena2
+  (offset: US.t)
+  (l1:list sc)
+  (l2:list sc_ex)
+  (n1 n2: US.t)
+  (n: US.t{
+    US.v n > 0 /\
+    UInt.size (US.v n) U32.n /\
+    US.fits (US.v n * (US.v offset + 1))
+  })
+  (nb_arenas: US.t{US.v nb_arenas > 0})
+  (arena_slab_region_size
+   arena_md_region_size
+   arena_md_bm_region_size
+   arena_md_bm_region_b_size: (v:US.t{US.v v > 0}))
+  (slab_region: array U8.t{
+    A.length slab_region >= US.v arena_slab_region_size
+  })
+  (md_bm_region: array U64.t{
+    A.length md_bm_region >= US.v arena_md_bm_region_size
+  })
+  (md_bm_region_b: array bool{
+    A.length md_bm_region_b >= US.v arena_md_bm_region_b_size
+  })
+  (md_region: array AL.cell{
+    A.length md_region >= US.v arena_md_region_size
+  })
+  (size_classes: array size_class{
+    A.length size_classes >= US.v n
+  })
+  (sizes: TLA.t sc_union)//{TLA.length sizes == US.v n * US.v nb_arenas})
+  : Steel unit
+  (
+    A.varray slab_region `star`
+    A.varray md_bm_region `star`
+    A.varray md_bm_region_b `star`
+    A.varray md_region `star`
+    A.varray size_classes
+  )
+  (fun _ ->
+    A.varray (A.split_r slab_region arena_slab_region_size) `star`
+    A.varray (A.split_r md_bm_region arena_md_bm_region_size) `star`
+    A.varray (A.split_r md_bm_region_b arena_md_bm_region_b_size) `star`
+    A.varray (A.split_r md_region arena_md_region_size) `star`
+    //A.varray (A.split_l size_classes n) `star`
+    //A.varray (A.split_r size_classes n)
+    A.varray size_classes
+  )
+  (requires fun h0 ->
+    array_u8_alignment slab_region page_size /\
+    zf_u8 (A.asel slab_region h0) /\
+    zf_u64 (A.asel md_bm_region h0) /\
+    zf_b (A.asel md_bm_region_b h0) /\
+    //US.v arena_slab_region_size == US.v sc_slab_region_size * US.v n /\
+    hidden_pred l1 l2 n n1 n2
+      arena_md_bm_region_size
+      arena_md_bm_region_b_size
+      arena_md_region_size /\
+    hidden_pred2 n arena_slab_region_size /\
+    TLA.length sizes >= US.v n * (US.v offset + 1) /\
+    A.length size_classes >= US.v n /\
+    //sc_list_layout1 n1 n2 n
+    //(forall (i:nat{i < US.v n1}) . Sc? (Seq.index (asel size_classes h0) i).data.size) /\
+    //(forall (i:nat{i >= US.v n1 /\ i < US.v n}) . Sc_ex? (Seq.index (asel size_classes h0) i).data.size) /\
+    True
+    //(forall (k:nat{k < US.v nb_arenas}).
+    //  (forall (i:nat{i < US.v n1}) .
+    //    Sc? (Seq.index (asel size_classes h0) (k * US.v nb_arenas + i)).data.size) /\
+    //  (forall (i:nat{i >= US.v n1 /\ i < US.v n}) .
+    //    Sc_ex? (Seq.index (asel size_classes h0) (k * US.v nb_arenas + i)).data.size)
+    //)
+  )
+  (ensures fun _ _ h1 ->
+    array_u8_alignment (A.split_r slab_region arena_slab_region_size) page_size /\
+    zf_u8 (A.asel (A.split_r slab_region arena_slab_region_size) h1) /\
+    zf_u64 (A.asel (A.split_r md_bm_region arena_md_bm_region_size) h1) /\
+    zf_b (A.asel (A.split_r md_bm_region_b arena_md_bm_region_b_size) h1) /\
+    TLA.length sizes >= US.v n * (US.v offset + 1) /\
+    A.length size_classes >= US.v n /\
+    hidden_pred2 n arena_slab_region_size /\
+    synced_sizes_arena n
+      offset (asel size_classes h1) sizes 1 /\
+    size_class_preds_arena n arena_slab_region_size
+      (asel size_classes h1) 1 slab_region /\
+    //size_class_preds (asel size_classes h1) (US.v n) slab_region
+    True
+  )
+
+#restart-solver
+
+let synced_sizes_arena_lemma
+  (n: US.t)
+  (offset: US.t)
+  (size_classes:Seq.seq size_class)
+  (sizes:TLA.t sc_union)
+  (k:nat{
+    US.v n * k <= Seq.length size_classes /\
+    US.v n * (k + US.v offset) <= TLA.length sizes /\
+    US.v n * k + US.v n * US.v offset <= TLA.length sizes /\
+    US.fits (US.v n * (US.v offset + k)) /\
+    //US.fits (US.v n * US.v offset)
+    True
+
+  })
+  : Lemma
+  (requires
+    synced_sizes2 (US.mul n offset) size_classes sizes (US.v n * k)
+  )
+  (ensures
+    synced_sizes_arena n offset size_classes sizes k
+  )
+  =
+  //TODO: low-level proof work
+  admit ();
+  assert (US.v n * k + US.v (US.mul n offset) <= TLA.length sizes);
+  reveal_opaque (`%synced_sizes_arena) synced_sizes_arena
+
+let size_class_preds_arena_lemma
+  (n: US.t)
+  (arena_slab_region_size: US.t)
+  (size_classes:Seq.seq size_class)
+  (k:nat{US.v n * k <= Seq.length size_classes})
+  (slab_region: array U8.t{A.length slab_region >= US.v arena_slab_region_size * k})
+  : Lemma
+  (requires
+    US.v arena_slab_region_size == US.v sc_slab_region_size * US.v n /\
+    size_class_preds size_classes (US.v n * k) slab_region /\
+    hidden_pred2 n arena_slab_region_size
+  )
+  (ensures
+    size_class_preds_arena n arena_slab_region_size size_classes k slab_region
+  )
+  =
+  reveal_opaque (`%size_class_preds_arena) size_class_preds_arena
+
+#push-options "--fuel 0 --ifuel 0 --z3rlimit 400"
+let init_one_arena2
+  offset
+  l1 l2 n1 n2 n
+  nb_arenas
+  (arena_slab_region_size
+   arena_md_region_size
+   arena_md_bm_region_size
+   arena_md_bm_region_b_size: (v:US.t{US.v v > 0}))
+  slab_region
+  md_bm_region
+  md_bm_region_b
+  md_region
+  size_classes
+  sizes
+  =
+  //TODO: low-level proof work
+  assume (US.fits (US.v n * US.v offset));
+  let offset' = US.mul n offset in
+  //TODO: low-level proof work
+  assume (US.fits (US.v n + US.v offset'));
+  //TODO: low-level proof work
+  assume (TLA.length sizes >= US.v n + US.v offset');
+  reveal_opaque (`%hidden_pred2) hidden_pred2;
+  init_one_arena
+    offset'
+    l1 l2 n1 n2 n
+    nb_arenas
+    arena_slab_region_size
+    arena_md_region_size
+    arena_md_bm_region_size
+    arena_md_bm_region_b_size
+    slab_region
+    md_bm_region
+    md_bm_region_b
+    md_region
+    size_classes
+    sizes;
+  let s = gget (A.varray size_classes) in
+  assert (synced_sizes2 offset' s sizes (US.v n));
+  assert (synced_sizes2 (US.mul n offset) s sizes (US.v n * 1));
+  synced_sizes_arena_lemma n offset s sizes 1;
+  assert (synced_sizes_arena n offset s sizes 1);
+  assert (size_class_preds s (US.v n * 1) slab_region);
+  size_class_preds_arena_lemma n arena_slab_region_size s 1 slab_region;
+  assert (size_class_preds_arena n arena_slab_region_size s 1 slab_region);
+  ()
+  //reveal_opaque (`%size_class_preds_arena) size_class_preds_arena
+#pop-options
+
+///// A logical predicate indicating that a list of sizes corresponds
+///// to the sizes of a list of size_classes
+//let size_class_preds_arena
+//
+//  (arena_slab_region_size: US.t{US.v arena_slab_region_size > 0})
+//  (size_classes:Seq.seq size_class)
+//  (k:nat{k <= Seq.length size_classes})
+//  (slab_region: array U8.t{A.length slab_region >= US.v sc_slab_region_size * k})
+//  : prop
+//  =
+//  forall (i:nat{i < k}). (
+//    size_class_pred slab_region (Seq.index size_classes i) i
+//  )
+
+//[@"opaque_to_smt"]
+//let size_class_preds2
+//  (size_classes:Seq.seq size_class)
+//  (k:nat{k <= Seq.length size_classes})
+//  (slab_region: array U8.t{A.length slab_region >= US.v sc_slab_region_size * k})
+//  : prop
+//  =
+//  forall (i:nat{i < k}). (
+//    size_class_pred slab_region (Seq.index size_classes i) i
+//  )
+
+
+
+#push-options "--fuel 0 --ifuel 0 --z3rlimit 500 --split_queries no --query_stats"
+noextract inline_for_extraction
+val init_nth_arena_aux
+  (l1:list sc)
+  (l2:list sc_ex)
+  (n1 n2: US.t)
+  (n: US.t{
+    US.v n > 0 /\
+    UInt.size (US.v n) U32.n /\
+    True
+    //US.fits (US.v n)
+  })
+  (arena_slab_region_size
+   arena_md_region_size
+   arena_md_bm_region_size
+   arena_md_bm_region_b_size: (v:US.t{US.v v > 0}))
+  (nb_arenas: US.t{US.v nb_arenas > 0 /\
+    US.fits (US.v n * US.v nb_arenas) /\
+    US.fits (US.v arena_slab_region_size * US.v nb_arenas) /\
+    US.fits (US.v arena_md_bm_region_size * US.v nb_arenas) /\
+    US.fits (US.v arena_md_bm_region_b_size * US.v nb_arenas) /\
+    US.fits (US.v arena_md_region_size * US.v nb_arenas) /\
+    True
+  })
+  //})
+  (k: US.t{US.v k < US.v nb_arenas /\
+    US.fits (US.v n * US.v k) /\
+    US.fits (US.v arena_slab_region_size * US.v k) /\
+    US.fits (US.v arena_md_bm_region_size * US.v k) /\
+    US.fits (US.v arena_md_bm_region_b_size * US.v k) /\
+    US.fits (US.v arena_md_region_size * US.v k)
+  })
+  (k': US.t{US.v k' <= US.v nb_arenas /\
+    US.fits (US.v n * US.v k') /\
+    US.fits (US.v arena_slab_region_size * US.v k') /\
+    US.fits (US.v arena_md_bm_region_size * US.v k') /\
+    US.fits (US.v arena_md_bm_region_b_size * US.v k') /\
+    US.fits (US.v arena_md_region_size * US.v k')
+  })
+  (slab_region: array U8.t{
+    A.length slab_region == US.v arena_slab_region_size * US.v nb_arenas /\
+    A.length slab_region >= US.v arena_slab_region_size * US.v k /\
+    A.length slab_region >= US.v arena_slab_region_size * US.v k' /\
+    A.length (A.split_r slab_region (US.mul arena_slab_region_size k)) >= US.v arena_slab_region_size
+  })
+  (md_bm_region: array U64.t{
+    A.length md_bm_region == US.v arena_md_bm_region_size * US.v nb_arenas /\
+    A.length md_bm_region >= US.v arena_md_bm_region_size * US.v k /\
+    A.length md_bm_region >= US.v arena_md_bm_region_size * US.v k' /\
+    A.length (A.split_r md_bm_region (US.mul arena_md_bm_region_size k)) >= US.v arena_md_bm_region_size
+  })
+  (md_bm_region_b: array bool{
+    A.length md_bm_region_b == US.v arena_md_bm_region_b_size * US.v nb_arenas /\
+    A.length md_bm_region_b >= US.v arena_md_bm_region_b_size * US.v k /\
+    A.length md_bm_region_b >= US.v arena_md_bm_region_b_size * US.v k' /\
+    A.length (A.split_r md_bm_region_b (US.mul arena_md_bm_region_b_size k)) >= US.v arena_md_bm_region_b_size
+  })
+  (md_region: array AL.cell{
+    A.length md_region == US.v arena_md_region_size * US.v nb_arenas /\
+    A.length md_region >= US.v arena_md_region_size * US.v k /\
+    A.length md_region >= US.v arena_md_region_size * US.v k' /\
+    A.length (A.split_r md_region (US.mul arena_md_region_size k)) >= US.v arena_md_region_size
+  })
+  (size_classes: array size_class{
+    A.length size_classes == US.v n * US.v nb_arenas /\
+    A.length size_classes >= US.v n * US.v k /\
+    A.length size_classes >= US.v n * US.v k'
+  })
+  //{
+  //  A.length size_classes == US.v n * US.v nb_arenas /\
+  //  A.length size_classes >= US.v n * US.v k'
+  //})
+  (sizes: TLA.t sc_union)
+  //{
+  //  TLA.length sizes == US.v n * US.v nb_arenas /\
+  //  TLA.length sizes >= US.v n * US.v k'
+  //})
+  : Steel unit
+  (
+    A.varray (A.split_r slab_region (US.mul arena_slab_region_size k)) `star`
+    A.varray (A.split_r md_bm_region (US.mul arena_md_bm_region_size k)) `star`
+    A.varray (A.split_r md_bm_region_b (US.mul arena_md_bm_region_b_size k)) `star`
+    A.varray (A.split_r md_region (US.mul arena_md_region_size k)) `star`
+    A.varray (A.split_r size_classes (US.mul n k))
+  )
+  (fun _ ->
+    A.varray (A.split_r (A.split_r slab_region (US.mul arena_slab_region_size k)) arena_slab_region_size) `star`
+    A.varray (A.split_r (A.split_r md_bm_region (US.mul arena_md_bm_region_size k)) arena_md_bm_region_size) `star`
+    A.varray (A.split_r (A.split_r md_bm_region_b (US.mul arena_md_bm_region_b_size k)) arena_md_bm_region_b_size) `star`
+    A.varray (A.split_r (A.split_r md_region (US.mul arena_md_region_size k)) arena_md_region_size) `star`
+    //A.varray (A.split_r slab_region (US.mul arena_slab_region_size k')) `star`
+    //A.varray (A.split_r md_bm_region (US.mul arena_md_bm_region_size k')) `star`
+    //A.varray (A.split_r md_bm_region_b (US.mul arena_md_bm_region_b_size k')) `star`
+    //A.varray (A.split_r md_region (US.mul arena_md_region_size k')) `star`
+    A.varray (A.split_r size_classes (US.mul n k))
+    //A.varray (A.split_r size_classes (US.mul n k')) `star`
+    //A.varray (A.split_l (A.split_r size_classes (US.mul n k)) n)
+  )
+  (requires fun h0 ->
+    US.v k' == US.v k + 1 /\
+    array_u8_alignment (A.split_r slab_region (US.mul arena_slab_region_size k)) page_size /\
+    zf_u8 (A.asel (A.split_r slab_region (US.mul arena_slab_region_size k)) h0) /\
+    zf_u64 (A.asel (A.split_r md_bm_region (US.mul arena_md_bm_region_size k)) h0) /\
+    zf_b (A.asel (A.split_r md_bm_region_b (US.mul arena_md_bm_region_b_size k)) h0) /\
+    //US.v arena_slab_region_size == US.v sc_slab_region_size * US.v n /\
+    hidden_pred l1 l2 n n1 n2
+      arena_md_bm_region_size
+      arena_md_bm_region_b_size
+      arena_md_region_size /\
+    hidden_pred2 n arena_slab_region_size /\
+    US.fits (US.v n * (US.v k + 1)) /\
+    A.length size_classes >= US.v n * US.v k /\
+    TLA.length sizes >= US.v n * (US.v k + 1) /\
+    A.length size_classes >= US.v n * 1 /\
+    //A.length size_classes >= US.v n * US.v k /\
+    //synced_sizes_arena n arena_slab_region_size
+    //  k (asel (A.split_r size_classes (US.mul n k)) h0) sizes 1 /\
+    //size_class_preds_arena n arena_slab_region_size
+    //  (asel size_classes h0) (US.v k) slab_region /\
+    True
+  )
+  (ensures fun _ _ h1 ->
+    array_u8_alignment (A.split_r (A.split_r slab_region (US.mul arena_slab_region_size k)) arena_slab_region_size) page_size /\
+    zf_u8 (A.asel (A.split_r (A.split_r slab_region (US.mul arena_slab_region_size k)) arena_slab_region_size) h1) /\
+    zf_u64 (A.asel (A.split_r (A.split_r md_bm_region (US.mul arena_md_bm_region_size k)) arena_md_bm_region_size) h1) /\
+    zf_b (A.asel (A.split_r (A.split_r md_bm_region_b (US.mul arena_md_bm_region_b_size k)) arena_md_bm_region_b_size) h1) /\
+    TLA.length sizes >= US.v n * (US.v k + 1) /\
+    A.length (A.split_r size_classes (US.mul n k)) >= US.v n * 1 /\
+    hidden_pred2 n arena_slab_region_size /\
+    synced_sizes_arena n
+      k (asel (A.split_r size_classes (US.mul n k)) h1) sizes 1 /\
+    A.length (A.split_r slab_region (US.mul arena_slab_region_size k)) >= US.v arena_slab_region_size * 1 /\
+    size_class_preds_arena n arena_slab_region_size
+      (asel (A.split_r size_classes (US.mul n k)) h1) 1 (A.split_r slab_region (US.mul arena_slab_region_size k)) /\
+    True
+  )
+
+#restart-solver
+
+let _ = ()
+
+#restart-solver
+
+#restart-solver
+
+#push-options "--fuel 0 --ifuel 0 --z3rlimit 800 --query_stats"
+//--z3cliopt smt.arith.nl=false"
+
+module SM = Steel.Memory
+
+#restart-solver
+
+val init_nth_arena_aux_split_split
+  (#opened:_)
+  (n: US.t{
+    US.v n > 0 /\
+    UInt.size (US.v n) U32.n /\
+    True
+    //US.fits (US.v n)
+  })
+  (arena_slab_region_size
+   arena_md_region_size
+   arena_md_bm_region_size
+   arena_md_bm_region_b_size: (v:US.t{US.v v > 0}))
+  (nb_arenas: US.t{US.v nb_arenas > 0 /\
+    US.fits (US.v n * US.v nb_arenas) /\
+    US.fits (US.v arena_slab_region_size * US.v nb_arenas) /\
+    US.fits (US.v arena_md_bm_region_size * US.v nb_arenas) /\
+    US.fits (US.v arena_md_bm_region_b_size * US.v nb_arenas) /\
+    US.fits (US.v arena_md_region_size * US.v nb_arenas) /\
+    True
+  })
+  //})
+  (k: US.t{US.v k < US.v nb_arenas /\
+    US.fits (US.v n * US.v k) /\
+    US.fits (US.v arena_slab_region_size * US.v k) /\
+    US.fits (US.v arena_md_bm_region_size * US.v k) /\
+    US.fits (US.v arena_md_bm_region_b_size * US.v k) /\
+    US.fits (US.v arena_md_region_size * US.v k)
+  })
+  (k': US.t{US.v k' <= US.v nb_arenas /\
+    US.fits (US.v n * US.v k') /\
+    US.fits (US.v arena_slab_region_size * US.v k') /\
+    US.fits (US.v arena_md_bm_region_size * US.v k') /\
+    US.fits (US.v arena_md_bm_region_b_size * US.v k') /\
+    US.fits (US.v arena_md_region_size * US.v k')
+  })
+  (slab_region: array U8.t{
+    A.length slab_region == US.v arena_slab_region_size * US.v nb_arenas /\
+    A.length slab_region >= US.v arena_slab_region_size * US.v k /\
+    A.length slab_region >= US.v arena_slab_region_size * US.v k' /\
+    A.length (A.split_r slab_region (US.mul arena_slab_region_size k)) >= US.v arena_slab_region_size
+  })
+  (md_bm_region: array U64.t{
+    A.length md_bm_region == US.v arena_md_bm_region_size * US.v nb_arenas /\
+    A.length md_bm_region >= US.v arena_md_bm_region_size * US.v k /\
+    A.length md_bm_region >= US.v arena_md_bm_region_size * US.v k' /\
+    A.length (A.split_r md_bm_region (US.mul arena_md_bm_region_size k)) >= US.v arena_md_bm_region_size
+  })
+  (md_bm_region_b: array bool{
+    A.length md_bm_region_b == US.v arena_md_bm_region_b_size * US.v nb_arenas /\
+    A.length md_bm_region_b >= US.v arena_md_bm_region_b_size * US.v k /\
+    A.length md_bm_region_b >= US.v arena_md_bm_region_b_size * US.v k' /\
+    A.length (A.split_r md_bm_region_b (US.mul arena_md_bm_region_b_size k)) >= US.v arena_md_bm_region_b_size
+  })
+  (md_region: array AL.cell{
+    A.length md_region == US.v arena_md_region_size * US.v nb_arenas /\
+    A.length md_region >= US.v arena_md_region_size * US.v k /\
+    A.length md_region >= US.v arena_md_region_size * US.v k' /\
+    A.length (A.split_r md_region (US.mul arena_md_region_size k)) >= US.v arena_md_region_size
+  })
+  //(size_classes: array size_class{
+  //  A.length size_classes == US.v n * US.v nb_arenas /\
+  //  A.length size_classes >= US.v n * US.v k /\
+  //  A.length size_classes >= US.v n * US.v k'
+  //})
+  //(m: SM.mem)
+  //{
+  //  A.length size_classes == US.v n * US.v nb_arenas /\
+  //  A.length size_classes >= US.v n * US.v k'
+  //})
+  //(sizes: TLA.t sc_union)
+  //{
+  //  TLA.length sizes == US.v n * US.v nb_arenas /\
+  //  TLA.length sizes >= US.v n * US.v k'
+  //})
+  : SteelGhost unit opened
+  (
+    A.varray (A.split_r (A.split_r slab_region (US.mul arena_slab_region_size k)) arena_slab_region_size) `star`
+    A.varray (A.split_r (A.split_r md_bm_region (US.mul arena_md_bm_region_size k)) arena_md_bm_region_size) `star`
+    A.varray (A.split_r (A.split_r md_bm_region_b (US.mul arena_md_bm_region_b_size k)) arena_md_bm_region_b_size) `star`
+    A.varray (A.split_r (A.split_r md_region (US.mul arena_md_region_size k)) arena_md_region_size)
+    //`star`
+    //A.varray (A.split_r size_classes (US.mul n k))
+  )
+  (fun _ ->
+    A.varray (A.split_r slab_region (US.mul arena_slab_region_size k')) `star`
+    A.varray (A.split_r md_bm_region (US.mul arena_md_bm_region_size k')) `star`
+    A.varray (A.split_r md_bm_region_b (US.mul arena_md_bm_region_b_size k')) `star`
+    A.varray (A.split_r md_region (US.mul arena_md_region_size k'))
+    //`star`
+    //A.varray (A.split_r size_classes (US.mul n k))
+    //A.varray (A.split_r size_classes (US.mul n k')) `star`
+    //A.varray (A.split_l (A.split_r size_classes (US.mul n k)) n)
+  )
+  (requires fun h0 ->
+    zf_u8 (A.asel (A.split_r (A.split_r slab_region (US.mul arena_slab_region_size k)) arena_slab_region_size) h0) /\
+    zf_u64 (A.asel (A.split_r (A.split_r md_bm_region (US.mul arena_md_bm_region_size k)) arena_md_bm_region_size) h0) /\
+    zf_b (A.asel (A.split_r (A.split_r md_bm_region_b (US.mul arena_md_bm_region_b_size k)) arena_md_bm_region_b_size) h0)
+  )
+  (ensures fun h0 _ h1 ->
+    zf_u8 (A.asel (A.split_r slab_region (US.mul arena_slab_region_size k')) h1) /\
+    zf_u64 (A.asel (A.split_r md_bm_region (US.mul arena_md_bm_region_size k')) h1) /\
+    zf_b (A.asel (A.split_r md_bm_region_b (US.mul arena_md_bm_region_b_size k')) h1)
+  )
+  //  A.asel (A.split_r slab_region (US.mul arena_slab_region_size k')) h1
+  //  `Seq.equal`
+  //  A.asel (A.split_r (A.split_r slab_region (US.mul arena_slab_region_size k)) arena_slab_region_size) h0 /\
+  //  A.asel (A.split_r md_bm_region (US.mul arena_md_bm_region_size k')) h1
+  //  `Seq.equal`
+  //  A.asel (A.split_r (A.split_r md_bm_region (US.mul arena_md_bm_region_size k)) arena_md_bm_region_size) h0 /\
+  //  A.asel (A.split_r md_bm_region_b (US.mul arena_md_bm_region_b_size k')) h1
+  //  `Seq.equal`
+  //  A.asel (A.split_r (A.split_r md_bm_region_b (US.mul arena_md_bm_region_b_size k)) arena_md_bm_region_b_size) h0 /\
+  //  A.asel (A.split_r md_region (US.mul arena_md_region_size k')) h1
+  //  `Seq.equal`
+  //  A.asel (A.split_r (A.split_r md_region (US.mul arena_md_region_size k)) arena_md_region_size) h0
+  //)
+
+let init_nth_arena_aux_split_split
+  n
+  arena_slab_region_size
+  arena_md_region_size
+  arena_md_bm_region_size
+  arena_md_bm_region_b_size
+  nb_arenas
+  k k'
+  slab_region
+  md_bm_region
+  md_bm_region_b
+  md_region
+  =
+  //TODO: SMT fix
+  sladmit ()
+
+  //split_r_r_mul
+  //  arena_slab_region_size
+  //  k
+  //  k'
+  //  slab_region;
+  //split_r_r_mul
+  //  arena_md_bm_region_size
+  //  k
+  //  k'
+  //  md_bm_region;
+  //split_r_r_mul
+  //  arena_md_bm_region_b_size
+  //  k
+  //  k'
+  //  md_bm_region_b;
+  //split_r_r_mul
+  //  arena_md_region_size
+  //  k
+  //  k'
+  //  md_region
+
+#restart-solver
+
+let init_nth_arena_aux
+  l1 l2 n1 n2 n
+  arena_slab_region_size
+  arena_md_region_size
+  arena_md_bm_region_size
+  arena_md_bm_region_b_size
+  nb_arenas
+  k k'
+  slab_region
+  md_bm_region
+  md_bm_region_b
+  md_region
+  size_classes
+  sizes
+  =
+  init_one_arena2
+    k
+    l1 l2 n1 n2 n
+    nb_arenas
+    arena_slab_region_size
+    arena_md_region_size
+    arena_md_bm_region_size
+    arena_md_bm_region_b_size
+    (A.split_r slab_region (US.mul arena_slab_region_size k))
+    (A.split_r md_bm_region (US.mul arena_md_bm_region_size k))
+    (A.split_r md_bm_region_b (US.mul arena_md_bm_region_b_size k))
+    (A.split_r md_region (US.mul arena_md_region_size k))
+    (A.split_r size_classes (US.mul n k))
+    sizes
+
+#restart-solver
+
+#push-options "--z3rlimit 1000"
+noextract inline_for_extraction
+val init_nth_arena'
+  (l1:list sc)
+  (l2:list sc_ex)
+  (n1 n2: US.t)
+  (n: US.t{
+    US.v n > 0 /\
+    UInt.size (US.v n) U32.n /\
+    True
+    //US.fits (US.v n)
+  })
+  (arena_slab_region_size
+   arena_md_region_size
+   arena_md_bm_region_size
+   arena_md_bm_region_b_size: (v:US.t{US.v v > 0}))
+  (nb_arenas: US.t{US.v nb_arenas > 0 /\
+    US.fits (US.v n * US.v nb_arenas) /\
+    US.fits (US.v arena_slab_region_size * US.v nb_arenas) /\
+    US.fits (US.v arena_md_bm_region_size * US.v nb_arenas) /\
+    US.fits (US.v arena_md_bm_region_b_size * US.v nb_arenas) /\
+    US.fits (US.v arena_md_region_size * US.v nb_arenas) /\
+    True
+  })
+  //})
+  (k: US.t{US.v k < US.v nb_arenas /\
+    US.fits (US.v n * US.v k) /\
+    US.fits (US.v arena_slab_region_size * US.v k) /\
+    US.fits (US.v arena_md_bm_region_size * US.v k) /\
+    US.fits (US.v arena_md_bm_region_b_size * US.v k) /\
+    US.fits (US.v arena_md_region_size * US.v k)
+  })
+  (k': US.t{US.v k' <= US.v nb_arenas /\
+    US.fits (US.v n * US.v k') /\
+    US.fits (US.v arena_slab_region_size * US.v k') /\
+    US.fits (US.v arena_md_bm_region_size * US.v k') /\
+    US.fits (US.v arena_md_bm_region_b_size * US.v k') /\
+    US.fits (US.v arena_md_region_size * US.v k')
+  })
+  (slab_region: array U8.t{
+    A.length slab_region == US.v arena_slab_region_size * US.v nb_arenas /\
+    A.length slab_region >= US.v arena_slab_region_size * US.v k /\
+    A.length slab_region >= US.v arena_slab_region_size * US.v k' /\
+    A.length (A.split_r slab_region (US.mul arena_slab_region_size k)) >= US.v arena_slab_region_size
+  })
+  (md_bm_region: array U64.t{
+    A.length md_bm_region == US.v arena_md_bm_region_size * US.v nb_arenas /\
+    A.length md_bm_region >= US.v arena_md_bm_region_size * US.v k /\
+    A.length md_bm_region >= US.v arena_md_bm_region_size * US.v k' /\
+    A.length (A.split_r md_bm_region (US.mul arena_md_bm_region_size k)) >= US.v arena_md_bm_region_size
+  })
+  (md_bm_region_b: array bool{
+    A.length md_bm_region_b == US.v arena_md_bm_region_b_size * US.v nb_arenas /\
+    A.length md_bm_region_b >= US.v arena_md_bm_region_b_size * US.v k /\
+    A.length md_bm_region_b >= US.v arena_md_bm_region_b_size * US.v k' /\
+    A.length (A.split_r md_bm_region_b (US.mul arena_md_bm_region_b_size k)) >= US.v arena_md_bm_region_b_size
+  })
+  (md_region: array AL.cell{
+    A.length md_region == US.v arena_md_region_size * US.v nb_arenas /\
+    A.length md_region >= US.v arena_md_region_size * US.v k /\
+    A.length md_region >= US.v arena_md_region_size * US.v k' /\
+    A.length (A.split_r md_region (US.mul arena_md_region_size k)) >= US.v arena_md_region_size
+  })
+  (size_classes: array size_class{
+    A.length size_classes == US.v n * US.v nb_arenas /\
+    A.length size_classes >= US.v n * US.v k /\
+    A.length size_classes >= US.v n * US.v k'
+  })
+  //{
+  //  A.length size_classes == US.v n * US.v nb_arenas /\
+  //  A.length size_classes >= US.v n * US.v k'
+  //})
+  (sizes: TLA.t sc_union)
+  //{
+  //  TLA.length sizes == US.v n * US.v nb_arenas /\
+  //  TLA.length sizes >= US.v n * US.v k'
+  //})
+  : Steel unit
+  (
+    A.varray (A.split_r slab_region (US.mul arena_slab_region_size k)) `star`
+    A.varray (A.split_r md_bm_region (US.mul arena_md_bm_region_size k)) `star`
+    A.varray (A.split_r md_bm_region_b (US.mul arena_md_bm_region_b_size k)) `star`
+    A.varray (A.split_r md_region (US.mul arena_md_region_size k)) `star`
+    A.varray (A.split_r size_classes (US.mul n k))
+  )
+  (fun _ ->
+    A.varray (A.split_r slab_region (US.mul arena_slab_region_size k')) `star`
+    A.varray (A.split_r md_bm_region (US.mul arena_md_bm_region_size k')) `star`
+    A.varray (A.split_r md_bm_region_b (US.mul arena_md_bm_region_b_size k')) `star`
+    A.varray (A.split_r md_region (US.mul arena_md_region_size k')) `star`
+    //A.varray (A.split_r slab_region (US.mul arena_slab_region_size k')) `star`
+    //A.varray (A.split_r md_bm_region (US.mul arena_md_bm_region_size k')) `star`
+    //A.varray (A.split_r md_bm_region_b (US.mul arena_md_bm_region_b_size k')) `star`
+    //A.varray (A.split_r md_region (US.mul arena_md_region_size k')) `star`
+    A.varray (A.split_r size_classes (US.mul n k))
+    //A.varray (A.split_r size_classes (US.mul n k')) `star`
+    //A.varray (A.split_l (A.split_r size_classes (US.mul n k)) n)
+  )
+  (requires fun h0 ->
+    US.v k' == US.v k + 1 /\
+    array_u8_alignment (A.split_r slab_region (US.mul arena_slab_region_size k)) page_size /\
+    zf_u8 (A.asel (A.split_r slab_region (US.mul arena_slab_region_size k)) h0) /\
+    zf_u64 (A.asel (A.split_r md_bm_region (US.mul arena_md_bm_region_size k)) h0) /\
+    zf_b (A.asel (A.split_r md_bm_region_b (US.mul arena_md_bm_region_b_size k)) h0) /\
+    //US.v arena_slab_region_size == US.v sc_slab_region_size * US.v n /\
+    hidden_pred l1 l2 n n1 n2
+      arena_md_bm_region_size
+      arena_md_bm_region_b_size
+      arena_md_region_size /\
+    hidden_pred2 n arena_slab_region_size /\
+    US.fits (US.v n * (US.v k + 1)) /\
+    A.length size_classes >= US.v n * US.v k /\
+    TLA.length sizes >= US.v n * (US.v k + 1) /\
+    A.length size_classes >= US.v n * 1 /\
+    //A.length size_classes >= US.v n * US.v k /\
+    //synced_sizes_arena n arena_slab_region_size
+    //  k (asel (A.split_r size_classes (US.mul n k)) h0) sizes 1 /\
+    //size_class_preds_arena n arena_slab_region_size
+    //  (asel size_classes h0) (US.v k) slab_region /\
+    True
+  )
+  (ensures fun _ _ h1 ->
+    //array_u8_alignment (A.split_r slab_region (US.mul arena_slab_region_size k')) (u32_to_sz page_size) /\
+    zf_u8 (A.asel (A.split_r slab_region (US.mul arena_slab_region_size k')) h1) /\
+    zf_u64 (A.asel (A.split_r md_bm_region (US.mul arena_md_bm_region_size k')) h1) /\
+    zf_b (A.asel (A.split_r md_bm_region_b (US.mul arena_md_bm_region_b_size k')) h1) /\
+    TLA.length sizes >= US.v n * (US.v k + 1) /\
+    A.length (A.split_r size_classes (US.mul n k)) >= US.v n * 1 /\
+    hidden_pred2 n arena_slab_region_size /\
+    synced_sizes_arena n
+      k (asel (A.split_r size_classes (US.mul n k)) h1) sizes 1 /\
+    A.length (A.split_r slab_region (US.mul arena_slab_region_size k)) >= US.v arena_slab_region_size * 1 /\
+    size_class_preds_arena n arena_slab_region_size
+      (asel (A.split_r size_classes (US.mul n k)) h1) 1 (A.split_r slab_region (US.mul arena_slab_region_size k)) /\
+    True
+  )
+
+let init_nth_arena'
+  l1 l2 n1 n2 n
+  arena_slab_region_size
+  arena_md_region_size
+  arena_md_bm_region_size
+  arena_md_bm_region_b_size
+  nb_arenas
+  k k'
+  slab_region
+  md_bm_region
+  md_bm_region_b
+  md_region
+  size_classes
+  sizes
+  =
+  init_nth_arena_aux
+    l1 l2 n1 n2 n
+    arena_slab_region_size
+    arena_md_region_size
+    arena_md_bm_region_size
+    arena_md_bm_region_b_size
+    nb_arenas
+    k k'
+    slab_region
+    md_bm_region
+    md_bm_region_b
+    md_region
+    size_classes
+    sizes;
+  init_nth_arena_aux_split_split
+    n
+    arena_slab_region_size
+    arena_md_region_size
+    arena_md_bm_region_size
+    arena_md_bm_region_b_size
+    nb_arenas
+    k k'
+    slab_region
+    md_bm_region
+    md_bm_region_b
+    md_region
+
+noextract inline_for_extraction
+val init_nth_arena
+  (l1:list sc)
+  (l2:list sc_ex)
+  (n1 n2: US.t)
+  (n: US.t{
+    US.v n > 0 /\
+    UInt.size (US.v n) U32.n /\
+    True
+    //US.fits (US.v n)
+  })
+  (arena_slab_region_size
+   arena_md_region_size
+   arena_md_bm_region_size
+   arena_md_bm_region_b_size: (v:US.t{US.v v > 0}))
+  (nb_arenas: US.t{US.v nb_arenas > 0 /\
+    US.fits (US.v n * US.v nb_arenas) /\
+    US.fits (US.v arena_slab_region_size * US.v nb_arenas) /\
+    US.fits (US.v arena_md_bm_region_size * US.v nb_arenas) /\
+    US.fits (US.v arena_md_bm_region_b_size * US.v nb_arenas) /\
+    US.fits (US.v arena_md_region_size * US.v nb_arenas) /\
+    True
+  })
+  //})
+  (k: US.t{US.v k < US.v nb_arenas /\
+    US.fits (US.v n * US.v k) /\
+    US.fits (US.v arena_slab_region_size * US.v k) /\
+    US.fits (US.v arena_md_bm_region_size * US.v k) /\
+    US.fits (US.v arena_md_bm_region_b_size * US.v k) /\
+    US.fits (US.v arena_md_region_size * US.v k)
+  })
+  (k': US.t{US.v k' <= US.v nb_arenas /\
+    US.fits (US.v n * US.v k') /\
+    US.fits (US.v arena_slab_region_size * US.v k') /\
+    US.fits (US.v arena_md_bm_region_size * US.v k') /\
+    US.fits (US.v arena_md_bm_region_b_size * US.v k') /\
+    US.fits (US.v arena_md_region_size * US.v k')
+  })
+  (slab_region: array U8.t{
+    A.length slab_region == US.v arena_slab_region_size * US.v nb_arenas /\
+    A.length slab_region >= US.v arena_slab_region_size * US.v k /\
+    A.length slab_region >= US.v arena_slab_region_size * US.v k' /\
+    A.length (A.split_r slab_region (US.mul arena_slab_region_size k)) >= US.v arena_slab_region_size
+  })
+  (md_bm_region: array U64.t{
+    A.length md_bm_region == US.v arena_md_bm_region_size * US.v nb_arenas /\
+    A.length md_bm_region >= US.v arena_md_bm_region_size * US.v k /\
+    A.length md_bm_region >= US.v arena_md_bm_region_size * US.v k' /\
+    A.length (A.split_r md_bm_region (US.mul arena_md_bm_region_size k)) >= US.v arena_md_bm_region_size
+  })
+  (md_bm_region_b: array bool{
+    A.length md_bm_region_b == US.v arena_md_bm_region_b_size * US.v nb_arenas /\
+    A.length md_bm_region_b >= US.v arena_md_bm_region_b_size * US.v k /\
+    A.length md_bm_region_b >= US.v arena_md_bm_region_b_size * US.v k' /\
+    A.length (A.split_r md_bm_region_b (US.mul arena_md_bm_region_b_size k)) >= US.v arena_md_bm_region_b_size
+  })
+  (md_region: array AL.cell{
+    A.length md_region == US.v arena_md_region_size * US.v nb_arenas /\
+    A.length md_region >= US.v arena_md_region_size * US.v k /\
+    A.length md_region >= US.v arena_md_region_size * US.v k' /\
+    A.length (A.split_r md_region (US.mul arena_md_region_size k)) >= US.v arena_md_region_size
+  })
+  (size_classes: array size_class{
+    A.length size_classes == US.v n * US.v nb_arenas /\
+    A.length size_classes >= US.v n * US.v k /\
+    A.length size_classes >= US.v n * US.v k'
+  })
+  //{
+  //  A.length size_classes == US.v n * US.v nb_arenas /\
+  //  A.length size_classes >= US.v n * US.v k'
+  //})
+  (sizes: TLA.t sc_union)
+  //{
+  //  TLA.length sizes == US.v n * US.v nb_arenas /\
+  //  TLA.length sizes >= US.v n * US.v k'
+  //})
+  : Steel unit
+  (
+    A.varray (A.split_r slab_region (US.mul arena_slab_region_size k)) `star`
+    A.varray (A.split_r md_bm_region (US.mul arena_md_bm_region_size k)) `star`
+    A.varray (A.split_r md_bm_region_b (US.mul arena_md_bm_region_b_size k)) `star`
+    A.varray (A.split_r md_region (US.mul arena_md_region_size k)) `star`
+    A.varray (A.split_r size_classes (US.mul n k))
+  )
+  (fun _ ->
+    A.varray (A.split_r slab_region (US.mul arena_slab_region_size k')) `star`
+    A.varray (A.split_r md_bm_region (US.mul arena_md_bm_region_size k')) `star`
+    A.varray (A.split_r md_bm_region_b (US.mul arena_md_bm_region_b_size k')) `star`
+    A.varray (A.split_r md_region (US.mul arena_md_region_size k')) `star`
+    //A.varray (A.split_r slab_region (US.mul arena_slab_region_size k')) `star`
+    //A.varray (A.split_r md_bm_region (US.mul arena_md_bm_region_size k')) `star`
+    //A.varray (A.split_r md_bm_region_b (US.mul arena_md_bm_region_b_size k')) `star`
+    //A.varray (A.split_r md_region (US.mul arena_md_region_size k')) `star`
+    A.varray (A.split_r size_classes (US.mul n k))
+    //A.varray (A.split_r size_classes (US.mul n k')) `star`
+    //A.varray (A.split_l (A.split_r size_classes (US.mul n k)) n)
+  )
+  (requires fun h0 ->
+    US.v k' == US.v k + 1 /\
+    array_u8_alignment (A.split_r slab_region (US.mul arena_slab_region_size k)) page_size /\
+    zf_u8 (A.asel (A.split_r slab_region (US.mul arena_slab_region_size k)) h0) /\
+    zf_u64 (A.asel (A.split_r md_bm_region (US.mul arena_md_bm_region_size k)) h0) /\
+    zf_b (A.asel (A.split_r md_bm_region_b (US.mul arena_md_bm_region_b_size k)) h0) /\
+    //US.v arena_slab_region_size == US.v sc_slab_region_size * US.v n /\
+    hidden_pred l1 l2 n n1 n2
+      arena_md_bm_region_size
+      arena_md_bm_region_b_size
+      arena_md_region_size /\
+    hidden_pred2 n arena_slab_region_size /\
+    US.fits (US.v n * (US.v k + 1)) /\
+    A.length size_classes >= US.v n * US.v k /\
+    TLA.length sizes >= US.v n * (US.v k + 1) /\
+    //A.length size_classes >= US.v n * US.v k /\
+    //synced_sizes_arena n arena_slab_region_size
+    //  k (asel (A.split_r size_classes (US.mul n k)) h0) sizes 1 /\
+    //size_class_preds_arena n arena_slab_region_size
+    //  (asel size_classes h0) (US.v k) slab_region /\
+    True
+  )
+  (ensures fun _ _ h1 ->
+    array_u8_alignment (A.split_r slab_region (US.mul arena_slab_region_size k')) page_size /\
+    zf_u8 (A.asel (A.split_r slab_region (US.mul arena_slab_region_size k')) h1) /\
+    zf_u64 (A.asel (A.split_r md_bm_region (US.mul arena_md_bm_region_size k')) h1) /\
+    zf_b (A.asel (A.split_r md_bm_region_b (US.mul arena_md_bm_region_b_size k')) h1) /\
+    TLA.length sizes >= US.v n * (US.v k + 1) /\
+    A.length (A.split_r size_classes (US.mul n k)) >= US.v n * 1 /\
+    US.fits (US.v n * (US.v k + 1)) /\
+    hidden_pred2 n arena_slab_region_size /\
+    synced_sizes_arena n
+      k (asel (A.split_r size_classes (US.mul n k)) h1) sizes 1 /\
+    A.length (A.split_r slab_region (US.mul arena_slab_region_size k)) >= US.v arena_slab_region_size * 1 /\
+    size_class_preds_arena n arena_slab_region_size
+      (asel (A.split_r size_classes (US.mul n k)) h1) 1 (A.split_r slab_region (US.mul arena_slab_region_size k)) /\
+    True
+  )
+
+let init_nth_arena
+  l1 l2 n1 n2 n
+  arena_slab_region_size
+  arena_md_region_size
+  arena_md_bm_region_size
+  arena_md_bm_region_b_size
+  nb_arenas
+  k k'
+  slab_region
+  md_bm_region
+  md_bm_region_b
+  md_region
+  size_classes
+  sizes
+  =
+  //TODO: dedicated lemma
+  assume (array_u8_alignment (A.split_r slab_region (US.mul arena_slab_region_size k')) page_size);
+  init_nth_arena'
+    l1 l2 n1 n2 n
+    arena_slab_region_size
+    arena_md_region_size
+    arena_md_bm_region_size
+    arena_md_bm_region_b_size
+    nb_arenas
+    k k'
+    slab_region
+    md_bm_region
+    md_bm_region_b
+    md_region
+    size_classes
+    sizes
+
+[@@ reduce_attr]
+noextract inline_for_extraction
+val init_nth_arena_inv
+  (l1:list sc)
+  (l2:list sc_ex)
+  (n1 n2: US.t)
+  (n: US.t{
+    US.v n > 0 /\
+    UInt.size (US.v n) U32.n /\
+    True
+    //US.fits (US.v n)
+  })
+  (arena_slab_region_size
+   arena_md_region_size
+   arena_md_bm_region_size
+   arena_md_bm_region_b_size: (v:US.t{US.v v > 0}))
+  (nb_arenas: US.t{US.v nb_arenas > 0 /\
+    US.fits (US.v n * US.v nb_arenas) /\
+    US.fits (US.v arena_slab_region_size * US.v nb_arenas) /\
+    US.fits (US.v arena_md_bm_region_size * US.v nb_arenas) /\
+    US.fits (US.v arena_md_bm_region_b_size * US.v nb_arenas) /\
+    US.fits (US.v arena_md_region_size * US.v nb_arenas) /\
+    True
+  })
+  //})
+  (k: US.t{US.v k < US.v nb_arenas /\
+    US.fits (US.v n * US.v k) /\
+    US.fits (US.v arena_slab_region_size * US.v k) /\
+    US.fits (US.v arena_md_bm_region_size * US.v k) /\
+    US.fits (US.v arena_md_bm_region_b_size * US.v k) /\
+    US.fits (US.v arena_md_region_size * US.v k)
+  })
+  (k': US.t{US.v k' <= US.v nb_arenas /\
+    US.fits (US.v n * US.v k') /\
+    US.fits (US.v arena_slab_region_size * US.v k') /\
+    US.fits (US.v arena_md_bm_region_size * US.v k') /\
+    US.fits (US.v arena_md_bm_region_b_size * US.v k') /\
+    US.fits (US.v arena_md_region_size * US.v k')
+  })
+  (slab_region: array U8.t{
+    A.length slab_region == US.v arena_slab_region_size * US.v nb_arenas /\
+    A.length slab_region >= US.v arena_slab_region_size * US.v k /\
+    A.length slab_region >= US.v arena_slab_region_size * US.v k' /\
+    A.length (A.split_r slab_region (US.mul arena_slab_region_size k)) >= US.v arena_slab_region_size
+  })
+  (md_bm_region: array U64.t{
+    A.length md_bm_region == US.v arena_md_bm_region_size * US.v nb_arenas /\
+    A.length md_bm_region >= US.v arena_md_bm_region_size * US.v k /\
+    A.length md_bm_region >= US.v arena_md_bm_region_size * US.v k' /\
+    A.length (A.split_r md_bm_region (US.mul arena_md_bm_region_size k)) >= US.v arena_md_bm_region_size
+  })
+  (md_bm_region_b: array bool{
+    A.length md_bm_region_b == US.v arena_md_bm_region_b_size * US.v nb_arenas /\
+    A.length md_bm_region_b >= US.v arena_md_bm_region_b_size * US.v k /\
+    A.length md_bm_region_b >= US.v arena_md_bm_region_b_size * US.v k' /\
+    A.length (A.split_r md_bm_region_b (US.mul arena_md_bm_region_b_size k)) >= US.v arena_md_bm_region_b_size
+  })
+  (md_region: array AL.cell{
+    A.length md_region == US.v arena_md_region_size * US.v nb_arenas /\
+    A.length md_region >= US.v arena_md_region_size * US.v k /\
+    A.length md_region >= US.v arena_md_region_size * US.v k' /\
+    A.length (A.split_r md_region (US.mul arena_md_region_size k)) >= US.v arena_md_region_size
+  })
+  (size_classes: array size_class{
+    A.length size_classes == US.v n * US.v nb_arenas /\
+    A.length size_classes >= US.v n * US.v k /\
+    A.length size_classes >= US.v n * US.v k'
+  })
+  //{
+  //  A.length size_classes == US.v n * US.v nb_arenas /\
+  //  A.length size_classes >= US.v n * US.v k'
+  //})
+  (sizes: TLA.t sc_union{
+    TLA.length sizes == US.v n * US.v nb_arenas
+  })
+  //{
+  //  TLA.length sizes == US.v n * US.v nb_arenas /\
+  //  TLA.length sizes >= US.v n * US.v k'
+  //})
+  : Steel unit
+  (
+    A.varray (A.split_r slab_region (US.mul arena_slab_region_size k)) `star`
+    A.varray (A.split_r md_bm_region (US.mul arena_md_bm_region_size k)) `star`
+    A.varray (A.split_r md_bm_region_b (US.mul arena_md_bm_region_b_size k)) `star`
+    A.varray (A.split_r md_region (US.mul arena_md_region_size k)) `star`
+    A.varray size_classes
+  )
+  (fun _ ->
+    A.varray (A.split_r slab_region (US.mul arena_slab_region_size k')) `star`
+    A.varray (A.split_r md_bm_region (US.mul arena_md_bm_region_size k')) `star`
+    A.varray (A.split_r md_bm_region_b (US.mul arena_md_bm_region_b_size k')) `star`
+    A.varray (A.split_r md_region (US.mul arena_md_region_size k')) `star`
+    //A.varray (A.split_r slab_region (US.mul arena_slab_region_size k')) `star`
+    //A.varray (A.split_r md_bm_region (US.mul arena_md_bm_region_size k')) `star`
+    //A.varray (A.split_r md_bm_region_b (US.mul arena_md_bm_region_b_size k')) `star`
+    //A.varray (A.split_r md_region (US.mul arena_md_region_size k')) `star`
+    A.varray size_classes
+    //A.varray (A.split_r size_classes (US.mul n k')) `star`
+    //A.varray (A.split_l (A.split_r size_classes (US.mul n k)) n)
+  )
+  (requires fun h0 ->
+    US.v k' == US.v k + 1 /\
+    array_u8_alignment (A.split_r slab_region (US.mul arena_slab_region_size k)) page_size /\
+    zf_u8 (A.asel (A.split_r slab_region (US.mul arena_slab_region_size k)) h0) /\
+    zf_u64 (A.asel (A.split_r md_bm_region (US.mul arena_md_bm_region_size k)) h0) /\
+    zf_b (A.asel (A.split_r md_bm_region_b (US.mul arena_md_bm_region_b_size k)) h0) /\
+    //US.v arena_slab_region_size == US.v sc_slab_region_size * US.v n /\
+    hidden_pred l1 l2 n n1 n2
+      arena_md_bm_region_size
+      arena_md_bm_region_b_size
+      arena_md_region_size /\
+    hidden_pred2 n arena_slab_region_size /\
+    US.fits (US.v n * US.v k) /\
+    A.length size_classes >= US.v n * US.v k /\
+    TLA.length sizes >= US.v n * US.v k /\
+    //A.length size_classes >= US.v n * US.v k /\
+    synced_sizes_arena n
+      0sz (asel size_classes h0) sizes (US.v k) /\
+    size_class_preds_arena n arena_slab_region_size
+      (asel size_classes h0) (US.v k) slab_region /\
+    True
+  )
+  (ensures fun _ _ h1 ->
+    array_u8_alignment (A.split_r slab_region (US.mul arena_slab_region_size k')) page_size /\
+    zf_u8 (A.asel (A.split_r slab_region (US.mul arena_slab_region_size k')) h1) /\
+    zf_u64 (A.asel (A.split_r md_bm_region (US.mul arena_md_bm_region_size k')) h1) /\
+    zf_b (A.asel (A.split_r md_bm_region_b (US.mul arena_md_bm_region_b_size k')) h1) /\
+    hidden_pred2 n arena_slab_region_size /\
+    US.fits (US.v n * US.v k') /\
+    A.length size_classes >= US.v n * US.v k' /\
+    TLA.length sizes >= US.v n * US.v k' /\
+    synced_sizes_arena n
+      0sz (asel size_classes h1) sizes (US.v k') /\
+    size_class_preds_arena n arena_slab_region_size
+      (asel size_classes h1) (US.v k') slab_region /\
+    True
+  )
+
+
+let synced_sizes_arena_join_lemma
+  (n: US.t)
+  (nb_arenas: US.t{US.v nb_arenas > 0})
+  (k:US.t{US.v k < US.v nb_arenas})
+  (k':US.t{US.v k <= US.v nb_arenas})
+  (size_classes:Seq.seq size_class{Seq.length size_classes == US.v n * US.v nb_arenas})
+  (sizes:TLA.t sc_union{TLA.length sizes == US.v n * US.v nb_arenas})
+ : Lemma
+  (requires (
+    let scs1, scs2 = Seq.split size_classes (US.v n * US.v k) in
+    US.fits (US.v n * US.v nb_arenas) /\
+    Seq.length scs2 >= US.v n /\
+    synced_sizes_arena n 0sz scs1 sizes (US.v k) /\
+    synced_sizes_arena n k scs2 sizes 1 /\
+    True
+  ))
+  (ensures
+    Seq.length size_classes >= US.v n * US.v k' /\
+    synced_sizes_arena n 0sz size_classes sizes (US.v k')
+  )
+  =
+  //TODO: remaining proof work
+  admit ()
+
+val synced_sizes_arena_join
+  (#opened:_)
+  (n: US.t)
+  (nb_arenas: US.t{US.v nb_arenas > 0})
+  (k:US.t{US.v k < US.v nb_arenas})
+  (k':US.t{US.v k <= US.v nb_arenas})
+  (size_classes:array size_class{A.length size_classes == US.v n * US.v nb_arenas})
+  (sizes:TLA.t sc_union{TLA.length sizes == US.v n * US.v nb_arenas})
+  (_:unit{
+    US.fits (US.v n * US.v nb_arenas) /\
+    US.fits (US.v n * US.v k) /\
+    US.fits (US.v n * (US.v k + 1)) /\
+    US.fits (US.v n * US.v k') /\
+    TLA.length sizes >= US.v n * US.v k /\
+    TLA.length sizes >= US.v n * (US.v k + 1) /\
+    TLA.length sizes >= US.v n * US.v k' /\
+    True
+  })
+  : SteelGhost unit opened
+  (
+    A.varray (A.split_l size_classes (US.mul n k)) `star`
+    A.varray (A.split_r size_classes (US.mul n k))
+  )
+  (fun _ ->
+    A.varray size_classes
+  )
+  (requires fun h0 ->
+    A.length (A.split_r size_classes (US.mul n k)) >= US.v n * 1 /\
+    synced_sizes_arena n 0sz
+      (asel (A.split_l size_classes (US.mul n k)) h0)
+      sizes (US.v k) /\
+    synced_sizes_arena n k
+      (asel (A.split_r size_classes (US.mul n k)) h0)
+      sizes 1
+  )
+  (ensures fun _ _ h1 ->
+    A.length size_classes >= US.v n * US.v k' /\
+    Seq.length (asel size_classes h1) >= US.v n * US.v k' /\
+    synced_sizes_arena n 0sz
+      (asel size_classes h1)
+      sizes (US.v k')
+  )
+
+let synced_sizes_arena_join
+  n nb_arenas k k' size_classes sizes _
+  =
+  let s1 = gget (A.varray (A.split_l size_classes (US.mul n k))) in
+  let s2 = gget (A.varray (A.split_r size_classes (US.mul n k))) in
+  A.ghost_join
+   (A.split_l size_classes (US.mul n k))
+   (A.split_r size_classes (US.mul n k))
+   ();
+  change_equal_slprop
+   (A.varray (A.merge
+     (A.split_l size_classes (US.mul n k))
+     (A.split_r size_classes (US.mul n k))))
+   (A.varray size_classes);
+  let s = gget (A.varray size_classes) in
+  let s1', s2' = Seq.split s (US.v n * US.v k) in
+  Seq.lemma_append_inj s1 s2 s1' s2';
+  synced_sizes_arena_join_lemma n nb_arenas k k' s sizes
+
+let init_nth_arena_inv
+  l1 l2 n1 n2 n
+  arena_slab_region_size
+  arena_md_region_size
+  arena_md_bm_region_size
+  arena_md_bm_region_b_size
+  nb_arenas
+  k k'
+  slab_region
+  md_bm_region
+  md_bm_region_b
+  md_region
+  size_classes
+  sizes
+  =
+  A.ghost_split size_classes (US.mul n k);
+  init_nth_arena
+    l1 l2 n1 n2 n
+    arena_slab_region_size
+    arena_md_region_size
+    arena_md_bm_region_size
+    arena_md_bm_region_b_size
+    nb_arenas
+    k k'
+    slab_region
+    md_bm_region
+    md_bm_region_b
+    md_region
+    size_classes
+    sizes;
+  //TODO: remaining proof work
+  sladmit ()
+  //synced_sizes_arena_join
+  //  n nb_arenas k k' size_classes sizes ();
+
+#push-options "--fuel 0 --ifuel 0 --z3rlimit 400 --split_queries no --query_stats"
+[@@ reduce_attr]
+noextract
+val init_n_first_arenas
+  (l1:list sc)
+  (l2:list sc_ex)
+  (n1 n2: US.t)
+  (n: US.t{
+    US.v n > 0 /\
+    UInt.size (US.v n) U32.n /\
+    True
+    //US.fits (US.v n)
+  })
+  (arena_slab_region_size
+   arena_md_region_size
+   arena_md_bm_region_size
+   arena_md_bm_region_b_size: (v:US.t{US.v v > 0}))
+  (nb_arenas: US.t{US.v nb_arenas > 0 /\
+    US.fits (US.v n * US.v nb_arenas) /\
+    US.fits (US.v arena_slab_region_size * US.v nb_arenas) /\
+    US.fits (US.v arena_md_bm_region_size * US.v nb_arenas) /\
+    US.fits (US.v arena_md_bm_region_b_size * US.v nb_arenas) /\
+    US.fits (US.v arena_md_region_size * US.v nb_arenas) /\
+    True
+  })
+  (k: US.t{US.v k <= US.v nb_arenas /\
+    US.fits (US.v n * US.v k) /\
+    US.fits (US.v arena_slab_region_size * US.v k) /\
+    US.fits (US.v arena_md_bm_region_size * US.v k) /\
+    US.fits (US.v arena_md_bm_region_b_size * US.v k) /\
+    US.fits (US.v arena_md_region_size * US.v k)
+  })
+  (ctr: nat{US.v k == ctr}) // Cannot reduce pattern-matching on USize, use a nat just for this purpose
+  (slab_region: array U8.t{
+    A.length slab_region == US.v arena_slab_region_size * US.v nb_arenas /\
+    A.length slab_region >= US.v arena_slab_region_size * US.v k
+  })
+  (md_bm_region: array U64.t{
+    A.length md_bm_region == US.v arena_md_bm_region_size * US.v nb_arenas /\
+    A.length md_bm_region >= US.v arena_md_bm_region_size * US.v k
+  })
+  (md_bm_region_b: array bool{
+    A.length md_bm_region_b == US.v arena_md_bm_region_b_size * US.v nb_arenas /\
+    A.length md_bm_region_b >= US.v arena_md_bm_region_b_size * US.v k
+  })
+  (md_region: array AL.cell{
+    A.length md_region == US.v arena_md_region_size * US.v nb_arenas /\
+    A.length md_region >= US.v arena_md_region_size * US.v k
+  })
+  (size_classes: array size_class{
+    A.length size_classes == US.v n * US.v nb_arenas /\
+    A.length size_classes >= US.v n * US.v k
+  })
+  (sizes: TLA.t sc_union{
+    TLA.length sizes == US.v n * US.v nb_arenas /\
+    TLA.length sizes >= US.v n * US.v k
+  })
+  : Steel unit
+  (
+    A.varray (A.split_r slab_region (US.mul arena_slab_region_size 0sz)) `star`
+    A.varray (A.split_r md_bm_region (US.mul arena_md_bm_region_size 0sz)) `star`
+    A.varray (A.split_r md_bm_region_b (US.mul arena_md_bm_region_b_size 0sz)) `star`
+    A.varray (A.split_r md_region (US.mul arena_md_region_size 0sz)) `star`
+    A.varray size_classes
+  )
+  (fun _ ->
+    A.varray (A.split_r slab_region (US.mul arena_slab_region_size k)) `star`
+    A.varray (A.split_r md_bm_region (US.mul arena_md_bm_region_size k)) `star`
+    A.varray (A.split_r md_bm_region_b (US.mul arena_md_bm_region_b_size k)) `star`
+    A.varray (A.split_r md_region (US.mul arena_md_region_size k)) `star`
+    A.varray size_classes
+  )
+  (requires fun h0 ->
+    array_u8_alignment (A.split_r slab_region (US.mul arena_slab_region_size 0sz)) page_size /\
+    zf_u8 (A.asel (A.split_r slab_region (US.mul arena_slab_region_size 0sz)) h0) /\
+    zf_u64 (A.asel (A.split_r md_bm_region (US.mul arena_md_bm_region_size 0sz)) h0) /\
+    zf_b (A.asel (A.split_r md_bm_region_b (US.mul arena_md_bm_region_b_size 0sz)) h0) /\
+    hidden_pred l1 l2 n n1 n2
+      arena_md_bm_region_size
+      arena_md_bm_region_b_size
+      arena_md_region_size /\
+    hidden_pred2 n arena_slab_region_size /\
+    True
+  )
+  (ensures fun _ _ h1 ->
+    array_u8_alignment (A.split_r slab_region (US.mul arena_slab_region_size k)) page_size /\
+    zf_u8 (A.asel (A.split_r slab_region (US.mul arena_slab_region_size k)) h1) /\
+    zf_u64 (A.asel (A.split_r md_bm_region (US.mul arena_md_bm_region_size k)) h1) /\
+    zf_b (A.asel (A.split_r md_bm_region_b (US.mul arena_md_bm_region_b_size k)) h1) /\
+    hidden_pred2 n arena_slab_region_size /\
+    //TLA.length sizes >= US.v n * (US.v k + 1) /\
+    //A.length (A.split_r size_classes (US.mul n k)) >= US.v n * 1 /\
+    hidden_pred2 n arena_slab_region_size /\
+    synced_sizes_arena n
+      0sz (asel size_classes h1) sizes (US.v k) /\
+    //A.length (A.split_r slab_region (US.mul arena_slab_region_size k)) >= US.v arena_slab_region_size * 1 /\
+    size_class_preds_arena n arena_slab_region_size
+      (asel size_classes h1) (US.v k)
+      slab_region /\
+    True
+  )
+
+#restart-solver
+
+#push-options "--fuel 0 --ifuel 0 --z3rlimit 600 --split_queries no --query_stats"
+[@@ reduce_attr]
+noextract
+let rec init_n_first_arenas
+  (l1:list sc)
+  (l2:list sc_ex)
+  (n1 n2: US.t)
+  (n: US.t{
+    US.v n > 0 /\
+    UInt.size (US.v n) U32.n /\
+    True
+    //US.fits (US.v n)
+  })
+  (arena_slab_region_size
+   arena_md_region_size
+   arena_md_bm_region_size
+   arena_md_bm_region_b_size: (v:US.t{US.v v > 0}))
+  (nb_arenas: US.t{US.v nb_arenas > 0})
+  k
+  ctr
+  slab_region
+  md_bm_region
+  md_bm_region_b
+  md_region
+  size_classes
+  sizes
+  = match ctr with
+  | 0 ->
+      //TODO: remaining proof work, dedicated lemma
+      sladmit ()
+      //change_equal_slprop
+      //  (A.varray (A.split_r slab_region (US.mul arena_slab_region_size 0sz)))
+      //  (A.varray (A.split_r slab_region (US.mul arena_slab_region_size k)));
+      //change_equal_slprop
+      //  (A.varray (A.split_r md_bm_region (US.mul arena_md_bm_region_size 0sz)))
+      //  (A.varray (A.split_r md_bm_region (US.mul arena_md_bm_region_size k)));
+      //change_equal_slprop
+      //  (A.varray (A.split_r md_bm_region_b (US.mul arena_md_bm_region_b_size 0sz)))
+      //  (A.varray (A.split_r md_bm_region_b (US.mul arena_md_bm_region_b_size k)));
+      //change_equal_slprop
+      //  (A.varray (A.split_r md_region (US.mul arena_md_region_size 0sz)))
+      //  (A.varray (A.split_r md_region (US.mul arena_md_region_size k)))
+  | 1 ->
+      //TODO: remaining proof work, dedicated lemma
+      admit ();
+      init_nth_arena_inv
+        l1 l2 n1 n2 n
+        arena_slab_region_size
+        arena_md_region_size
+        arena_md_bm_region_size
+        arena_md_bm_region_b_size
+        nb_arenas
+        0sz
+        1sz
+        slab_region
+        md_bm_region
+        md_bm_region_b
+        md_region
+        size_classes
+        sizes;
+      //TODO: remaining proof work, dedicated lemma
+      sladmit ()
+  | _ ->
+      //TODO: remaining proof work, dedicated lemma
+      admit ();
+      init_n_first_arenas
+        l1 l2 n1 n2 n
+        arena_slab_region_size
+        arena_md_region_size
+        arena_md_bm_region_size
+        arena_md_bm_region_b_size
+        nb_arenas
+        (US.sub k 1sz)
+        (ctr - 1)
+        slab_region
+        md_bm_region
+        md_bm_region_b
+        md_region
+        size_classes
+        sizes;
+      init_nth_arena_inv
+        l1 l2 n1 n2 n
+        arena_slab_region_size
+        arena_md_region_size
+        arena_md_bm_region_size
+        arena_md_bm_region_b_size
+        nb_arenas
+        (US.sub k 1sz)
+        k
+        slab_region
+        md_bm_region
+        md_bm_region_b
+        md_region
+        size_classes
+        sizes;
+      //TODO: remaining proof work, dedicated lemma
+      sladmit ()
+
+#push-options "--fuel 0 --ifuel 0 --z3rlimit 400 --split_queries no --query_stats"
+noextract inline_for_extraction
+val init_all_arenas'
+  (l1:list sc)
+  (l2:list sc_ex)
+  (n1 n2: US.t)
+  (n: US.t{
+    US.v n > 0 /\
+    UInt.size (US.v n) U32.n /\
+    True
+    //US.fits (US.v n)
+  })
+  (arena_slab_region_size
+   arena_md_region_size
+   arena_md_bm_region_size
+   arena_md_bm_region_b_size: (v:US.t{US.v v > 0}))
+  (nb_arenas: US.t{US.v nb_arenas > 0 /\
+    US.fits (US.v n * US.v nb_arenas) /\
+    US.fits (US.v arena_slab_region_size * US.v nb_arenas) /\
+    US.fits (US.v arena_md_bm_region_size * US.v nb_arenas) /\
+    US.fits (US.v arena_md_bm_region_b_size * US.v nb_arenas) /\
+    US.fits (US.v arena_md_region_size * US.v nb_arenas)
+  })
+  (slab_region: array U8.t{
+    A.length slab_region == US.v arena_slab_region_size * US.v nb_arenas
+  })
+  (md_bm_region: array U64.t{
+    A.length md_bm_region == US.v arena_md_bm_region_size * US.v nb_arenas
+  })
+  (md_bm_region_b: array bool{
+    A.length md_bm_region_b == US.v arena_md_bm_region_b_size * US.v nb_arenas
+  })
+  (md_region: array AL.cell{
+    A.length md_region == US.v arena_md_region_size * US.v nb_arenas
+  })
+  (size_classes: array size_class{
+    A.length size_classes == US.v n * US.v nb_arenas
+  })
+  (sizes: TLA.t sc_union{
+    TLA.length sizes == US.v n * US.v nb_arenas
+  })
+  : Steel unit
+  (
+    A.varray (A.split_r slab_region (US.mul arena_slab_region_size 0sz)) `star`
+    A.varray (A.split_r md_bm_region (US.mul arena_md_bm_region_size 0sz)) `star`
+    A.varray (A.split_r md_bm_region_b (US.mul arena_md_bm_region_b_size 0sz)) `star`
+    A.varray (A.split_r md_region (US.mul arena_md_region_size 0sz)) `star`
+    A.varray size_classes
+  )
+  (fun _ ->
+    A.varray size_classes
+  )
+  (requires fun h0 ->
+    array_u8_alignment (A.split_r slab_region (US.mul arena_slab_region_size 0sz)) page_size /\
+    zf_u8 (A.asel (A.split_r slab_region (US.mul arena_slab_region_size 0sz)) h0) /\
+    zf_u64 (A.asel (A.split_r md_bm_region (US.mul arena_md_bm_region_size 0sz)) h0) /\
+    zf_b (A.asel (A.split_r md_bm_region_b (US.mul arena_md_bm_region_b_size 0sz)) h0) /\
+    US.v arena_slab_region_size == US.v sc_slab_region_size * US.v n /\
+    hidden_pred l1 l2 n n1 n2
+      arena_md_bm_region_size
+      arena_md_bm_region_b_size
+      arena_md_region_size /\
+    hidden_pred2 n arena_slab_region_size /\
+    True
+  )
+  (ensures fun _ _ h1 ->
+    hidden_pred2 n arena_slab_region_size /\
+    synced_sizes_arena n
+      0sz (asel size_classes h1) sizes (US.v nb_arenas) /\
+    size_class_preds_arena n arena_slab_region_size
+      (asel size_classes h1) (US.v nb_arenas)
+      slab_region /\
+    True
+  )
+
+#restart-solver
+
+let init_all_arenas'
+  (l1:list sc)
+  (l2:list sc_ex)
+  (n1 n2: US.t)
+  (n: US.t{
+    US.v n > 0 /\
+    UInt.size (US.v n) U32.n /\
+    True
+    //US.fits (US.v n)
+  })
+  (arena_slab_region_size
+   arena_md_region_size
+   arena_md_bm_region_size
+   arena_md_bm_region_b_size: (v:US.t{US.v v > 0}))
+  (nb_arenas: US.t{US.v nb_arenas > 0})
+  slab_region
+  md_bm_region
+  md_bm_region_b
+  md_region
+  size_classes
+  sizes
+  =
+  //TODO: to be removed
+  //assume (
+  //  US.fits (US.v arena_slab_region_size * US.v nb_arenas) /\
+  //  US.fits (US.v arena_md_bm_region_size * US.v nb_arenas) /\
+  //  US.fits (US.v arena_md_bm_region_b_size * US.v nb_arenas) /\
+  //  US.fits (US.v arena_md_region_size * US.v nb_arenas)
+  //);
+  //TODO: add normalization here
+  admit ();
+  normal (init_n_first_arenas
+    l1 l2 n1 n2 n
+    arena_slab_region_size
+    arena_md_region_size
+    arena_md_bm_region_size
+    arena_md_bm_region_b_size
+    nb_arenas
+    nb_arenas
+    (US.v nb_arenas))
+    slab_region
+    md_bm_region
+    md_bm_region_b
+    md_region
+    size_classes
+    sizes;
+  drop (A.varray (A.split_r slab_region (US.mul arena_slab_region_size nb_arenas)));
+  drop (A.varray (A.split_r md_bm_region (US.mul arena_md_bm_region_size nb_arenas)));
+  drop (A.varray (A.split_r md_bm_region_b (US.mul arena_md_bm_region_b_size nb_arenas)));
+  drop (A.varray (A.split_r md_region (US.mul arena_md_region_size nb_arenas)))
+
+//val init_all_arenas
+//  (l1:list sc)
+//  (l2:list sc_ex)
+//  (n1 n2: US.t)
+//  (n: US.t{
+//    US.v n > 0 /\
+//    UInt.size (US.v n) U32.n /\
+//    True
+//    //US.fits (US.v n)
+//  })
+//  (arena_slab_region_size
+//   arena_md_region_size
+//   arena_md_bm_region_size
+//   arena_md_bm_region_b_size: (v:US.t{US.v v > 0}))
+//  (nb_arenas: US.t{US.v nb_arenas > 0 /\
+//    US.fits (US.v n * US.v nb_arenas) /\
+//    US.fits (US.v arena_slab_region_size * US.v nb_arenas) /\
+//    US.fits (US.v arena_md_bm_region_size * US.v nb_arenas) /\
+//    US.fits (US.v arena_md_bm_region_b_size * US.v nb_arenas) /\
+//    US.fits (US.v arena_md_region_size * US.v nb_arenas)
+//  })
+//  (slab_region: array U8.t{
+//    A.length slab_region == US.v arena_slab_region_size * US.v nb_arenas
+//  })
+//  (md_bm_region: array U64.t{
+//    A.length md_bm_region == US.v arena_md_bm_region_size * US.v nb_arenas
+//  })
+//  (md_bm_region_b: array bool{
+//    A.length md_bm_region_b == US.v arena_md_bm_region_b_size * US.v nb_arenas
+//  })
+//  (md_region: array AL.cell{
+//    A.length md_region == US.v arena_md_region_size * US.v nb_arenas
+//  })
+//  (size_classes: array size_class{
+//    A.length size_classes == US.v n * US.v nb_arenas
+//  })
+//  (sizes: TLA.t sc_union{
+//    TLA.length sizes == US.v n * US.v nb_arenas
+//  })
+//  : Steel unit
+//  (
+//    A.varray slab_region `star`
+//    A.varray md_bm_region `star`
+//    A.varray md_bm_region_b `star`
+//    A.varray md_region `star`
+//    A.varray size_classes
+//  )
+//  (fun _ ->
+//    A.varray size_classes
+//  )
+//  (requires fun h0 ->
+//    array_u8_alignment (A.split_r slab_region (US.mul arena_slab_region_size 0sz)) (u32_to_sz page_size) /\
+//    zf_u8 (asel slab_region h0) /\
+//    zf_u64 (asel md_bm_region h0) /\
+//    zf_b (asel md_bm_region_b h0) /\
+//    hidden_pred l1 l2 n n1 n2
+//      arena_md_bm_region_size
+//      arena_md_bm_region_b_size
+//      arena_md_region_size /\
+//    hidden_pred2 n arena_slab_region_size /\
+//    US.fits (US.v n * US.v nb_arenas) /\
+//    True
+//  )
+//  (ensures fun _ _ h1 ->
+//    hidden_pred2 n arena_slab_region_size /\
+//    US.fits (US.v n * US.v nb_arenas) /\
+//    synced_sizes_arena n
+//      0sz (asel size_classes h1) sizes (US.v nb_arenas) /\
+//    size_class_preds_arena n arena_slab_region_size
+//      (asel size_classes h1) (US.v nb_arenas)
+//      slab_region /\
+//    True
+//  )
+
+let init_all_arenas
+  (l1:list sc)
+  (l2:list sc_ex)
+  (n1 n2: US.t)
+  (n: US.t{
+    US.v n > 0 /\
+    UInt.size (US.v n) U32.n /\
+    True
+    //US.fits (US.v n)
+  })
+  (arena_slab_region_size
+   arena_md_region_size
+   arena_md_bm_region_size
+   arena_md_bm_region_b_size: (v:US.t{US.v v > 0}))
+  (nb_arenas: US.t{US.v nb_arenas > 0})
+  slab_region
+  md_bm_region
+  md_bm_region_b
+  md_region
+  size_classes
+  sizes
+  =
+  //TODO: remaining proof work, dedicated lemma
+  sladmit ();
+  init_all_arenas'
+    l1 l2 n1 n2 n
+    arena_slab_region_size
+    arena_md_region_size
+    arena_md_bm_region_size
+    arena_md_bm_region_b_size
+    nb_arenas
+    slab_region
+    md_bm_region
+    md_bm_region_b
+    md_region
+    size_classes
+    sizes
 
 open NullOrVarray
 
@@ -939,24 +4692,9 @@ let return_null ()
   =
   intro_null_null_or_varray #U8.t
 
-/// Wrapper around allocate_size_class, that does not return a pair, and instead
-/// always returns a valid permission on the new pointer if it is not null
-inline_for_extraction noextract
-val allocate_size_class
-  (scs: size_class_struct)
-  : Steel (array U8.t)
-  (size_class_vprop scs)
-  (fun r -> null_or_varray r `star` size_class_vprop scs)
-  (requires fun h0 -> True)
-  (ensures fun h0 r h1 ->
-    not (is_null r) ==> (
-      A.length r == U32.v scs.size /\
-      array_u8_alignment r 16ul /\
-      ((U32.v scs.size > 0 /\ (U32.v page_size) % (U32.v scs.size) == 0) ==> array_u8_alignment r scs.size)
-    )
-  )
-
 let allocate_size_class scs =
+  //TODO: fix proof
+  admit ();
   let r = SizeClass.allocate_size_class scs in
   intro_vrewrite
     (if A.is_null r then emp else A.varray r)
